- Added all of the compatibility lemmas for the new logical relation which are parametric on the bounds invariants - Progress on generic closure conversion proof w.r.t. the explicit heap allocation + gc semantics - Cleaned up old closure conversion proof, factored out reusable lemmas

theories/L6_PCPS/Heap/cc_log_rel.v
@@ -9,37 +9,34 @@ From L6 Require Import functions cps eval cps_util identifiers ctx Ensembles_uti
                        List_util Heap.heap Heap.heap_defs Heap.space_sem.
 From Libraries Require Import Coqlib.
 
+Import ListNotations.
+
 Module CC_log_rel (H : Heap).
 
   Module Sem := SpaceSem H.
 
   Import H Sem.Defs Sem.
 
-  (* Global invariant *)
+  (** Global invariant *)
   Definition GInv :=
     nat -> (* The step index *)
-    relation (exp * env * heap val * nat * nat).
+    relation (heap block * env * exp * nat * nat).
   
-  (* Local invariant *)
+  (** Local invariant *)
+  (* XXX Same type as the GInv. Merge them at some point *)
   Definition Inv :=
-    relation (nat * nat).
-  
-  (* Tag for closure records *)
+    nat -> (* The step index *)
+    relation (heap block * env * exp * nat * nat).
+
+  (** Initial invariant *)
+  Definition IInv :=
+    relation (heap block * env * exp).
+
+  (** Tag for closure records *)
   Variable (clo_tag : cTag). 
 
-  Inductive fundefs_Forall2
-            (R : var -> fTag -> list var -> exp -> var -> fTag -> list var -> exp -> Prop)
-  : fundefs -> fundefs -> Prop :=
-  | Forall2_Fcons :
-      forall f1 ft1 xs1 e1 B1 f2 ft2 xs2 e2 B2, 
-        fundefs_Forall2 R B1 B2 ->
-        R f1 ft1 xs1 e1 f2 ft2 xs2 e2 ->
-        fundefs_Forall2 R (Fcons f1 ft1 xs1 e1 B1) (Fcons f2 ft2 xs2 e2 B2)
-  | Forall2_Fnil :
-      fundefs_Forall2 R Fnil Fnil.
-
   (** step-indexed relation on cps terms. Relates cps-terms with closure-converted terms  *)
-  (* Expression relation : 
+  (* Expression relation : (XXX This comment is not up-to-date)
    * ---------------------
    *  (e1, ρ1, H1) ~_k (e2, ρ2, H2) iff 
    *    forall c1 <= k,
@@ -60,211 +57,238 @@ Module CC_log_rel (H : Heap).
    *                (e2, [x2 -> l2', f2 -> l_clo, Γ -> l_env], H2)
    * else True (* ? -- not quite sure yet *)
    *)
-  Fixpoint cc_approx_val (k : nat) (P : GInv) (r1 r2 : res) {struct k} : Prop :=
-    let cc_approx_exp (k : nat) (p1 p2 : exp * env * heap val) : Prop :=
-        let '(e1, rho1, H1) := p1 in
-        let '(e2, rho2, H2) := p2 in
-        forall r1 c1 m1,
-          c1 <= k ->
-          big_step_perfect_GC H1 rho1 e1 r1 c1 m1 ->
-          exists r2 c2 m2,
-            big_step_perfect_GC H2 rho2 e2 r2 c2 m2 /\
-            P k (e1, rho1, H1, c1, m1) (e2, rho2, H2, c2, m2) /\
-            cc_approx_val (k - c1) P r1 r2
-    in
-    let '(l1, H1) := r1 in
-    let '(l2, H2) := r2 in 
-    match get l1 H1 with
-      | Some v1 =>
-        match get l2 H2 with
-          | Some v2 =>
-            match v1, v2 with
-              | Vfun rho1 defs1,
-                Vconstr tag (l_clo :: l_env :: l)  =>
-                exists rho2 defs2, 
-                  get l_clo H2 = Some (Vfun rho2 defs2) /\
-                  fundefs_Forall2
-                    (fun f1 ft1 xs1 e1 f2 ft2 xs2 e2 =>
-                       forall (ls1 ls2 : list loc) (j : nat) (rho1' : env),
-                         length ls1 = length ls2 ->
-                         Some rho1' = setlist xs1 ls1 (def_funs defs1 l1 rho1) ->
-                         exists (rho2' : env),
-                           tag = clo_tag /\
-                           Some rho2' = setlist xs2 (l_env :: ls2)
-                                                (def_funs defs2 l2 rho2) /\
-                           match k with
-                             | 0 => True
-                             | S k =>
-                               let R l1 l2 := cc_approx_val (k - (k-j)) P (l1, H1) (l2, H2) in
-                               j < S k ->
-                               Forall2 R ls1 ls2 ->
-                               cc_approx_exp (k - (k - j)) (e1, rho1', H1) (e2, rho2', H2)
-                           end
-                    ) defs1 defs2
-              | Vconstr t1 ls1, Vconstr t2 ls2 =>
-                t1 = t2 /\ 
-                match k with
-                  | 0 => True
-                  | S k =>
-                    let R l1 l2 := cc_approx_val k P (l1, H1) (l2, H2) in
-                    Forall2 R ls1 ls2
-                end
-              | _, _ => False
-            end
-          | None => False
-        end
-      | None => get l2 H2 = None (* ? *)
-    end.
 
-  Definition cc_approx_exp (k : nat) (P1 : Inv) (P2 : GInv)
-             (p1 p2 : exp * env * heap val) : Prop :=
-    let '(e1, rho1, H1) := p1 in
-    let '(e2, rho2, H2) := p2 in
-    forall r1 c1 m1,
-      c1 <= k ->
-      big_step_perfect_GC H1 rho1 e1 r1 c1 m1 ->
-      exists r2 c2 m2,
-        big_step_perfect_GC H2 rho2 e2 r2 c2 m2 /\
-        (* extra invariants for costs *)
-        P1 (c1, m1) (c2, m2) /\
-        cc_approx_val (k - c1) P2 r1 r2.
+
+  (** Definitions parametric on the value relation *)
+  Section cc_approx.
+    
+    Variable (cc_approx_val : nat -> GInv -> res -> res -> Prop). 
+
+    (** * Expression relation *)
+
+    Definition cc_approx_exp (k : nat) (P1 : Inv ) (P2 : GInv)
+               (p1 p2 : exp * env * heap block) : Prop :=
+      let '(e1, rho1, H1) := p1 in
+      let '(e2, rho2, H2) := p2 in
+      forall (H1' H2' : heap block) (r1 : res) (c1 m1 : nat),
+        reach' H1 (env_locs rho1 (occurs_free e1)) |- H1 ≡ H1' ->
+        reach' H2 (env_locs rho2 (occurs_free e2)) |- H2 ≡ H2' ->
+        c1 <= k ->
+        big_step_perfect_GC H1' rho1 e1 r1 c1 m1 ->
+        exists (r2 : res) (c2 m2 : nat),
+          big_step_perfect_GC H2' rho2 e2 r2 c2 m2 /\
+          (* extra invariants for costs *)
+          P1 k (H1', rho1, e1, c1, m1) (H2', rho2, e2, c2, m2) /\
+          cc_approx_val (k - c1) P2 r1 r2.
+    
+  End cc_approx.
   
-  (** More compact definition of the value relation *)
-  Definition cc_approx_val' (k : nat) (P : GInv) (r1 r2 : res) : Prop :=
-    let '(l1, H1) := r1 in
-    let '(l2, H2) := r2 in 
-    match get l1 H1 with
-      | Some v1 =>
-        match get l2 H2 with
-          | Some v2 =>
-            match v1, v2 with
-              | Vfun rho1 defs1, Vconstr tag (l_clo :: l_env :: l) =>
-                exists rho2 defs2, 
-                  get l_clo H2 = Some (Vfun rho2 defs2) /\
-                  fundefs_Forall2
-                    (fun f1 ft1 xs1 e1 f2 ft2 xs2 e2 =>
-                       forall (ls1 ls2 : list loc) (j : nat) (rho1' : env),
-                         length ls1 = length ls2 ->
-                         Some rho1' = setlist xs1 ls1 (def_funs defs1 l1 rho1) ->
-                         exists (rho2' : env),
-                           tag = clo_tag /\
-                           Some rho2' = setlist xs2 (l_env :: ls2)
-                                                (def_funs defs2 l2 rho2) /\
-                           (j < k ->
-                            Forall2 (fun l1 l2 => cc_approx_val j P (l1, H1) (l2, H2))
-                                    ls1 ls2 ->
-                            cc_approx_exp j (fun p1 p2 =>
-                                               let '(c1, m1) := p1 in
-                                               let '(c2, m2) := p2 in
-                                               P j
-                                                 (e1, rho1', H1, c1, m1)
-                                                 (e2, rho2', H2, c2, m2))
-                                          P (e1, rho1', H1) (e2, rho2', H2))
-                    ) defs1 defs2
-              | Vconstr t1 ls1, Vconstr t2 ls2 =>
-                t1 = t2 /\ 
-                match k with
-                  | 0 => True
-                  | S k =>
-                    let R l1 l2 := cc_approx_val k P (l1, H1) (l2, H2) in
-                    Forall2 R ls1 ls2
-                end
-              | _, _ => False
-            end
-          | None => False
-        end
-      | None => get l2 H2 = None
+  (** * Value relation *)
+
+  Fixpoint cc_approx_val (k : nat) (P : GInv) (r1 r2 : res) {struct k} : Prop :=
+    let '(v1, H1) := r1 in
+    let '(v2, H2) := r2 in
+    match v1, v2 with
+      | Loc l1, Loc l2 =>
+        exists c (vs1 vs2 : list value),
+          get l1 H1 = Some (Vconstr c vs1) /\
+          get l2 H2 = Some (Vconstr c vs2) /\
+          match k with
+            | 0 => True
+            | S k =>
+              let R l1 l2 := cc_approx_val k P (l1, H1) (l2, H2) in
+              Forall2 R vs1 vs2
+          end
+      | FunPtr lf1 f1, Loc l2 =>
+        exists rho1 B1 lf2 f2 venv rho2 B2,
+          get lf1 H1 = Some (Vfun rho1 B1) /\
+          get l2 H2 = Some (Vconstr clo_tag [(FunPtr lf2 f2) ; venv]) /\
+          get lf2 H2 = Some (Vfun rho2 B2) /\
+          forall (xs1 : list var) (ft : fTag) (e1 : exp)
+            (rho1' : env) (vs1 vs2 : list value) (j : nat),
+            find_def f1 B1 = Some (ft, xs1, e1) ->
+            length vs1 = length vs2 ->
+            Some rho1' = setlist xs1 vs1 (def_funs B1 lf1 rho1) ->
+            exists (xs2 : list var) (e2 : exp) (rho2' : env),
+              find_def f2 B2 = Some (ft, xs2, e2) /\
+              Some rho2' = setlist xs2 (venv :: vs2) (def_funs B2 lf2 rho2) /\
+              match k with
+                | 0 => True
+                | S k =>
+                  j < S k ->
+                  (forall H1' H2',
+                     let R v1 v2 := cc_approx_val (k - (k - j)) P (v1, H1') (v2, H2') in
+                     reach' H1 [set lf1] |- H1 ≡ H1' ->
+                     reach' H2 [set l2] |- H2 ≡ H2' ->
+                     Forall2 R vs1 vs2 ->
+                     cc_approx_exp cc_approx_val
+                                   (k - (k - j))
+                                   P P 
+                                   (e1, rho1', H1') (e2, rho2', H2'))
+              end
+      | _, _ => False
     end.
+  
 
-  Lemma fundefs_Forall2_monotonic
-        (R1 R2 : var -> fTag -> list var -> exp -> var -> fTag -> list var -> exp -> Prop) B1 B2:
-    (forall f1 ft1 xs1 e1 f2 ft2 xs2 e2,
-       R1 f1 ft1 xs1 e1 f2 ft2 xs2 e2 -> R2 f1 ft1 xs1 e1 f2 ft2 xs2 e2) ->
-    fundefs_Forall2 R1 B1 B2 ->
-    fundefs_Forall2 R2 B1 B2.
-  Proof.
-    intros Hyp Hdefs. induction Hdefs; constructor; eauto.
-  Qed.
-
+  (** Notations for approximation relations *)
+  Notation "p1 ⪯ ^ ( k ; P1 ; P2 ) p2" :=
+    (cc_approx_exp cc_approx_val k P1 P2 p1 p2)
+      (at level 70, no associativity).
+  
+  (** Unfold the recursion. A more compact definition of the value relation. *)
+  Definition cc_approx_val' (k : nat) (P : GInv) (r1 r2 : res) : Prop :=
+    let '(v1, H1) := r1 in
+    let '(v2, H2) := r2 in
+    match v1, v2 with
+      | Loc l1, Loc l2 =>
+        exists (c : cTag) (vs1 vs2 : list value),
+          get l1 H1 = Some (Vconstr c vs1) /\
+          get l2 H2 = Some (Vconstr c vs2) /\
+          match k with
+            | 0 => True
+            | S k =>
+              let R l1 l2 := cc_approx_val k P (l1, H1) (l2, H2) in
+              Forall2 R vs1 vs2
+          end
+      | FunPtr lf1 f1, Loc l2 =>
+        exists rho1 B1 lf2 f2 v_env rho2 B2,
+          get lf1 H1 = Some (Vfun rho1 B1) /\
+          get l2 H2 = Some (Vconstr clo_tag [(FunPtr lf2 f2) ; v_env]) /\
+          get lf2 H2 = Some (Vfun rho2 B2) /\
+          forall (xs1 : list var) (ft : fTag) (e1 : exp)
+            (rho1' : env) (vs1 vs2 : list value) (j : nat),
+            find_def f1 B1 = Some (ft, xs1, e1) ->
+            length vs1 = length vs2 ->
+            Some rho1' = setlist xs1 vs1 (def_funs B1 lf1 rho1) ->
+            exists (xs2 : list var) (e2 : exp) (rho2' : env),
+              find_def f2 B2 = Some (ft, xs2, e2) /\
+              Some rho2' = setlist xs2 (v_env :: vs2) (def_funs B2 lf2 rho2) /\
+              (j < k ->
+               forall H1' H2',
+                 reach' H1 [set lf1] |- H1 ≡ H1' ->
+                 reach' H2 [set l2] |- H2 ≡ H2' ->
+                 Forall2 (fun v1 v2 => cc_approx_val j P (v1, H1') (v2, H2')) vs1 vs2 ->
+                 (e1, rho1', H1') ⪯ ^ (j ; P ; P) (e2, rho2', H2'))
+      | _, _ => False
+    end.
+  
   (** Correspondence of the two definitions *)
   Lemma cc_approx_val_eq (k : nat) P (v1 v2 : res) :
     cc_approx_val k P v1 v2 <-> cc_approx_val' k P v1 v2.
   Proof.
-    destruct k as [ | k ]; destruct v1 as (l1, H1); destruct v2 as (l2, H2). simpl.
-    - destruct (get l1 H1) as [v1 | ] eqn:Hget1;
-      destruct (get l2 H2) as [v2 | ] eqn:Hget2; try now firstorder.
-      destruct v1; destruct v2;
-      eauto; try (split; intros H; (now simpl in H; inv H)).
-      + destruct l; [ now firstorder |].
-        destruct l0; [ now firstorder |].
-        split; intros [rho2 [defs2 [Hget Hyp]]]; do 2 eexists; (split; [ eassumption |  ]).
-        * eapply fundefs_Forall2_monotonic; [| eassumption ].
-          intros. edestruct H as [? [? [? ?]]]; eauto.
-          eexists; repeat split; eauto. intros; omega.
-        * eapply fundefs_Forall2_monotonic; [| eassumption ].
-          intros ? ? ? ? ? ? ? ? H ? ? ? ? ? ?.
-          edestruct H with (j := 0) as [? [? [? ? ]]]; eauto.
-    - simpl; destruct (get l1 H1) as [v1 | ] eqn:Hget1;
-      destruct (get l2 H2) as [v2 | ] eqn:Hget2; try now firstorder.
-      destruct v1; destruct v2;
-      eauto; try (split; intros H; (now simpl in H; inv H)). 
-      + destruct l; [ now firstorder |].
-        destruct l0; [ now firstorder |].
-        split; intros [rho2 [defs2 [Hget Hyp]]]; do 2 eexists; (split; [ eassumption |  ]).
-        * eapply fundefs_Forall2_monotonic; [| eassumption ].
-          intros. edestruct H with (j := j) as [? [? [? Hyp']]]; eauto.
-          subst.
-          eexists x; repeat split; eauto. intros.
-          assert (Heq : k - (k - j) = j) by omega. rewrite <- Heq.
-          eapply Hyp'; eauto; [| omega ]. rewrite Heq. eassumption.
-        *  eapply fundefs_Forall2_monotonic; [| eassumption ].
-          intros. edestruct H with (j := j) as [? [? [? Hyp']]]; eauto.
-          subst. eexists x; repeat split; eauto. intros.
-          assert (Heq : k - (k - j) = j) by omega. rewrite Heq.
-          eapply Hyp'; eauto; [| omega ]. rewrite <- Heq. eassumption.
+    destruct k as [ | k ];
+    destruct v1 as [[l1 | lf1 f1] H1]; destruct v2 as [[l2 | lf2 f2] H2];
+    try (now split; intros; contradiction).
+    - split; intros [c [vs1 [vs2 [Hget1 [Hget2 _]]]]]; repeat eexists; eauto.
+    - split;
+      (intros Hyp;
+       destruct Hyp
+         as (rho1 & B1 & lf2 & f2 & v_env & rho2 & B2 & Hget & Hgetl2 & Hgetlf2  & Hyp');
+       do 7 eexists; split; [ | split; [| split ] ]; (try now eauto);
+       intros xs1 ft e1 rho1' vs1 vs2 j Hfind Hlen Hset;
+       destruct (Hyp' xs1 ft e1 rho1' vs1 vs2 j Hfind Hlen Hset)
+         as (xs2 & e2 & rho2' & Hfind' & Hset' & HT);
+       do 3 eexists; repeat split; now eauto). 
+    - split; intros [c [vs1 [vs2 [Hget1 [Hget2 Hall]]]]]; repeat eexists; eauto.
+    - split;
+      (intros Hyp;
+       destruct Hyp
+         as (rho1 & B1 & lf2 & f2 & v_env & rho2 & B2 & Hget & Hgetl2 & Hgetlf2  & Hyp');
+       do 7 eexists; split; [ | split; [| split ] ]; (try now eauto);
+       intros xs1 ft e1 rho1' vs1 vs2 j Hfind Hlen Hset;
+       destruct (Hyp' xs1 ft e1 rho1' vs1 vs2 j Hfind Hlen Hset)
+         as (xs2 & e2 & rho2' & Hfind' & Hset' & Hi);
+       do 3 eexists; repeat split; try now eauto).
+      intros Hlt H1' H2' HH1 HH2 Hall.
+      assert (Heq : k - (k - j) = j) by omega. rewrite !Heq in Hi.
+      eapply Hi. omega. eassumption. eassumption. eassumption.
+      intros Hlt H1' H2' R HH1 HH2 Hall.
+      assert (Heq : k - (k - j) = j) by omega. unfold R in *. rewrite !Heq in *.
+      eapply Hi. omega. eassumption. eassumption. eassumption.
   Qed.
-
+  
   Opaque cc_approx_val.
 
+  (** * Environment relations *)
+  
   (** Environment relation for a single point (i.e. variable) : 
    * ρ1 ~_k^x ρ2 iff ρ1(x) = Some v -> ρ2(x) = Some v' /\ v ~_k v' *)
-  Definition cc_approx_var_env (k : nat) P (H1 : heap val) (rho1 : env)
-             (H2 : heap val) (rho2 : env) (x y : var) : Prop :=
+  Definition cc_approx_var_env (k : nat) P (H1 : heap block) (rho1 : env)
+             (H2 : heap block) (rho2 : env) (x y : var) : Prop :=
     forall l1, 
       M.get x rho1 = Some l1 -> 
       exists l2, M.get y rho2 = Some l2 /\
             cc_approx_val' k P (l1, H1) (l2, H2).
-
+  
   (** Environment relation for a set of points (i.e. predicate over variables) :
     * ρ1 ~_k^S ρ2 iff 
     *  forall x, S x -> ρ1(x) = Some v -> ρ2(x) = Some v' /\ v ~_k v' *)
-  Definition cc_approx_env_P (S : Ensemble var) k P (c1 c2 : heap val * env) :=
+  Definition cc_approx_env_P (S : Ensemble var) k P (c1 c2 : heap block * env) :=
     let (H1, rho1) := c1 in
     let (H2, rho2) := c2 in
     forall (x : var), S x -> cc_approx_var_env k P H1 rho1 H2 rho2 x x.
   
+  Notation "p1 ≺ ^ ( k ; P ) p2" := (cc_approx_val' k P p1 p2)
+                                      (at level 70, no associativity).
+
+  Notation "p1 ⋞ ^ ( R ; k ; P ) p2" := (cc_approx_env_P R k P p1 p2)
+                                          (at level 70, no associativity).
+
+  
   (** Environment relation for the whole domain of definition :
     * ρ1 ~_k ρ2 iff forall x, ρ1(x) = v => ρ2(x) = v' /\ v ~_k v' *)
   Definition cc_approx_env (k : nat) P c1 c2 : Prop :=
-    cc_approx_env_P (fun _ => True) k P c1 c2.
+    c1 ⋞ ^ (Full_set _; k; P) c2.
 
-  (** Notations for approximation relations *)
+  (** * Environment Invariants for Closure Conversion *)
 
-  Notation "p1 ⪯ ^ ( k ; P1 ; P2 ) p2" := (cc_approx_exp k P1 P2 p1 p2)
-                                            (at level 70, no associativity).
+  (** Naming conventions in the following :
+
+    [Scope] : The set of variables in the current scope.
+
+    [Funs] : The set of variables in the current block of mutually recursive
+    functions.
+
+    [FVs] : The list of free variables (needs to be ordered).
+
+    [Γ] : The formal parameter of the environment after closure conversion. *)
   
-
-  Notation "p1 ≺ ^ ( k ; P ) p2" := (cc_approx_val' k P p1 p2)
-                              (at level 70, no associativity).
+  (** Invariant about the free variables *) 
+  Definition FV_inv (k : nat) (P : GInv)
+             (rho1 : env) (H1 : heap block) (rho2 : env) (H2 : heap block)
+             (Scope Funs : Ensemble var) (c : cTag) (Γ : var) (FVs : list var) : Prop :=
+    forall (x : var) N (v : value),
+      ~ In _ Scope x ->
+      ~ In _ Funs x -> 
+      nthN FVs N = Some x ->
+      M.get x rho1 = Some v ->
+      exists (vs : list value) (l : loc) (v' : value),
+        M.get Γ rho2 = Some (Loc l) /\
+        get l H2 = Some (Vconstr c vs) /\
+        nthN vs N = Some v' /\
+        (v, H1) ≺ ^ ( k ; P ) (v', H2).
   
-  Notation "p1 ⋞ ^ ( R ; k ; P ) p2" := (cc_approx_env_P R k P p1 p2)
-                                          (at level 70, no associativity).
+  (** Invariant about the functions in the current function definition *)
+  Definition Fun_inv (k : nat) (P : GInv)
+             (rho1 : env) (H1 : heap block) (rho2 : env) (H2 : heap block)
+             (Scope Funs : Ensemble var) (σ : var -> var) (c : cTag) (Γ : var)  : Prop :=
+    forall (f : var) (vf1 : value),
+      ~ In _ Scope f ->
+      In var Funs f ->
+      M.get f rho1 = Some vf1 ->
+      exists (vf1 venv : value),
+        ~ In _ Scope (σ f) /\
+        M.get (σ f) rho2 = Some vf1 /\
+        M.get Γ rho2 = Some venv /\
+        forall l_clo vs,
+          get l_clo H1 = Some (Vconstr c (vf1 :: venv :: vs)) ->
+          (vf1, H1) ≺ ^ ( k ; P ) (Loc l_clo, H2).
   
   (** * Monotonicity Properties *)
 
   (** The environment relation is antimonotonic in the set of free variables *) 
   Lemma cc_approx_env_P_antimon (S1 S2 : Ensemble var) (k : nat)
-        (P : GInv) (c1 c2 : (heap val) * env) :
+        (P : GInv) (c1 c2 : (heap block) * env) :
     c1 ⋞ ^ ( S2 ; k ; P ) c2 ->
     S1 \subset S2 ->
     c1 ⋞ ^ ( S1 ; k ; P ) c2.
@@ -274,18 +298,20 @@ Module CC_log_rel (H : Heap).
   Qed.
   
   (** The expression relation is monotonic in the local invariant *)
-  Lemma cc_approx_exp_rel_mon k (P1 P1' : Inv) P2 p1 p2 :
+  Lemma cc_approx_exp_rel_mon k (P1 P1' : Inv) (P2 : GInv) p1 p2 :
     p1 ⪯ ^ ( k ; P1 ; P2 ) p2 ->
-    inclusion _ P1 P1' ->
+    (forall i, inclusion _ (P1 i) (P1' i)) ->
     p1 ⪯ ^ ( k ; P1' ; P2 ) p2.
   Proof.
     destruct p1 as [[e1 H1] rho1].
     destruct p2 as [[e2 H2] rho2].
-    intros Hcc Hin v1 c1 m1 Hleq Hstep.
+    intros Hcc Hin H1' H2' v1 c1 m1 HH1 HH2 Hleq Hstep.
     edestruct Hcc as [v2 [c2 [m2 [Hstep' [HInv Hval]]]]]; eauto.
-    repeat eexists; eauto.
+    repeat eexists; eauto. eapply Hin. eassumption.
   Qed.
-  
+
+  (** The logical relation respects equivalence of the global invariant *)
+
   Lemma cc_approx_exp_same_rel_IH k (P1 : Inv) (P2 P2' : GInv) p1 p2 :
     (forall m r1 r2,
        m <= k ->
@@ -297,14 +323,14 @@ Module CC_log_rel (H : Heap).
   Proof.
     destruct p1 as [[e1 H1] rho1].
     destruct p2 as [[e2 H2] rho2].
-    intros IH Hcc Hin v1 c1 m1 Hleq Hstep.
+    intros IH Hcc Hin H1' H2' v1 c1 m1 HH1 HH2 Hleq Hstep.
     edestruct Hcc as [v2 [c2 [m2 [Hstep2 [HP Hval]]]]]; eauto.
     repeat eexists; eauto.
     rewrite cc_approx_val_eq.
     eapply IH; eauto. omega.
     rewrite <- cc_approx_val_eq; eauto.    
   Qed.
-
+  
   Opaque cc_approx_exp.
 
   Lemma cc_approx_val_same_rel (k : nat) (P1 P2 : GInv) r1 r2 :
@@ -312,50 +338,42 @@ Module CC_log_rel (H : Heap).
     (forall n, same_relation _ (P1 n) (P2 n)) ->
     r1 ≺ ^ (k; P2) r2.
   Proof.
-    revert k P1 P2 r1 r2.
-    induction k using lt_wf_rec1.
-    intros P1 P2 r1 r2 Hv1 Hrel.
-    destruct r1 as (l1, H1); destruct r2 as (l2, H2).
-    destruct k; simpl in *.
-    - destruct (get l1 H1) as [v1 | ] eqn:Hget1;
-      destruct (get l2 H2) as [v2 | ] eqn:Hget2;
-      try congruence.
-      destruct v1; destruct v2;
-      eauto; try (split; intros H; (now simpl in H; inv H)).
-      destruct l; [ now firstorder |].
-      destruct l0; [ now firstorder |].
-      destruct Hv1 as [rho2 [defs2 [Hget Hyp]]];
-        do 2 eexists; (split; [ eassumption |  ]).
-      eapply fundefs_Forall2_monotonic; [| eassumption ].
-      intros. edestruct H0 with (j := 0)as [? [? [? ?]]]; eauto.
-      eexists; repeat split; eauto. intros; omega.
-    - destruct (get l1 H1) as [v1 | ] eqn:Hget1;
-      destruct (get l2 H2) as [v2 | ] eqn:Hget2;
-      try congruence.
-      destruct v1; destruct v2;
-      eauto; try (split; intros H; (now simpl in H; inv H)).
-      + destruct Hv1 as [Heq Hall]; subst.
-        split; eauto. eapply Forall2_monotonic; [| eassumption ].
-        intros; eauto. rewrite cc_approx_val_eq.
-        eapply H; eauto. rewrite <- cc_approx_val_eq; eauto.
-      + destruct l; [ now firstorder |].
-        destruct l0; [ now firstorder |].
-        destruct Hv1 as [rho2 [defs2 [Hget Hyp]]];
-          do 2 eexists; (split; [ eassumption |  ]).
-        eapply fundefs_Forall2_monotonic; [| eassumption ]. simpl.
-        intros ? ? ? ? ? ? ? ? Hypj. intros.
-        edestruct Hypj with (j := j) as [? [? [? Hval]]]; eauto.
-        eexists; repeat split; eauto. intros ? ?. 
-        eapply cc_approx_exp_same_rel_IH with (P2 := P1) (P2' := P2). 
-        intros; eapply H. omega. eassumption. eassumption.
-        eapply cc_approx_exp_rel_mon. eapply Hval; eauto.
+    revert k P1 P2 r1 r2. induction k as [k IHk] using lt_wf_rec1.
+    intros P1 P2 r1 r2 Hyp HR.
+    destruct k as [ | k ];
+    destruct r1 as [[l1 | lf1 f1] H1]; destruct r2 as [[l2 | lf2 f2] H2]; simpl;
+    try (now intros; contradiction).
+    - destruct Hyp as [c [vs1 [vs2 [Hget1 [Hget2 Hall]]]]]; repeat eexists; eauto.
+    - destruct Hyp
+        as (rho1 & B1 & lf2 & f2 & v_env & rho2 & B2 & Hget & Hgetl2 & Hgetlf2  & Hyp');
+      do 7 eexists; split; [ | split; [| split ] ]; (try now eauto);
+      intros xs1 ft e1 rho1' vs1 vs2 j Hfind Hlen Hset;
+      destruct (Hyp' xs1 ft e1 rho1' vs1 vs2 j Hfind Hlen Hset)
+        as (xs2 & e2 & rho2' & Hfind' & Hset' & HT);
+      do 3 eexists; repeat split; now eauto.
+    - destruct Hyp as [c [vs1 [vs2 [Hget1 [Hget2 Hall]]]]]; repeat eexists; eauto.
+      eapply Forall2_monotonic; [| eassumption ].
+      intros. rewrite cc_approx_val_eq in *. eapply IHk; eauto. 
+    - destruct Hyp
+        as (rho1 & B1 & lf2 & f2 & v_env & rho2 & B2 & Hget & Hgetl2 & Hgetlf2 & Hyp');
+      do 7 eexists; split; [ | split; [| split ] ]; (try now eauto);
+      intros xs1 ft e1 rho1' vs1 vs2 j Hfind Hlen Hset;
+      destruct (Hyp' xs1 ft e1 rho1' vs1 vs2 j Hfind Hlen Hset)
+        as (xs2 & e2 & rho2' & Hfind' & Hset' & Hi);
+      do 3 eexists; repeat split; try now eauto.
+      intros Hlt H1' H2' HH1 HH2 Hall.
+      eapply cc_approx_exp_same_rel_IH with (P2 := P1) (P2' := P2);
+        try eassumption. 
+      + intros; eapply IHk. omega. eassumption. eassumption.
+      + eapply cc_approx_exp_rel_mon. eapply Hi; eauto.
         eapply Forall2_monotonic; [| eassumption ].
         intros. rewrite cc_approx_val_eq.
-        eapply H; eauto. now rewrite <- cc_approx_val_eq; simpl in *; eauto.
-        intros. now firstorder.
-        intros [? ?] [? ?]. now firstorder. now firstorder.
+        eapply IHk; eauto. now rewrite <- cc_approx_val_eq; simpl in *; eauto.
+        now intros n; destruct (HR n); split; eauto.
+        intros i [[[[? ?] ?] ?] ?] [[[[? ?] ?] ?] ?] HP1. eapply HR.
+        eassumption.
   Qed.
-
+  
   Transparent cc_approx_exp.
 
   Lemma cc_approx_exp_same_rel (P : relation nat) k (P1 : Inv) (P2 P2' : GInv)
@@ -367,53 +385,70 @@ Module CC_log_rel (H : Heap).
     intros Hcc Hin. eapply cc_approx_exp_same_rel_IH; try eassumption.
     intros. eapply cc_approx_val_same_rel; eauto.
   Qed.
-
-  (** The value relation is monotonic in the step index *)
-  Lemma cc_approx_val_monotonic (k j : nat) (P : GInv) (r1 r2 : res) :
-    r1 ≺ ^ (k; P) r2 ->
-    j <= k ->
-    r1 ≺ ^ (j; P) r2.
-  Proof.
-    revert j P r1 r2. induction k as [k IHk] using lt_wf_rec1.
-    intros j P [l1 H1] [l2 H2] Hv1 Hleq.
-    simpl in *;
-      destruct (get l1 H1) as [v1 | ] eqn:Hget1;
-      destruct (get l2 H2) as [v2 | ] eqn:Hget2;
-    try congruence.
-    destruct v1; destruct v2;
-    eauto; try (split; intros H; (now simpl in H; inv H)).
-    - destruct Hv1 as [Heq Hall].
-      destruct j as [| j]; eauto. destruct k as [| k]; try omega.
-      split; eauto. eapply Forall2_monotonic; [| eassumption ].
-      intros. rewrite cc_approx_val_eq in *.
-      simpl in H. eapply IHk; [| eassumption |]; omega.
-    - destruct l; [ now firstorder |].
-      destruct l0; [ now firstorder |].
-      destruct Hv1 as [rho2 [defs2 [Hget Hyp]]];
-      do 2 eexists; (split; [ eassumption |  ]).
-      eapply fundefs_Forall2_monotonic; [| eassumption ].
-      intros.
-      edestruct H with (j := j0) as [rho2' [? [? Hypj]]]; eauto.
-      eexists; repeat split; eauto. intros.
-      edestruct Hypj as [r2 [c2 [m2 [Hbs [HP Hcc]]]]]; eauto.
-      omega. repeat eexists; eauto.
-  Qed.
-
-  (** The expression relation is monotonic in the step index *)
-  Lemma cc_approx_exp_monotonic (k j : nat) (P1 : Inv) (P2 : GInv)
-        p1 p2 :
-    p1 ⪯ ^ ( k ; P1 ; P2 ) p2 ->
-    j <= k ->
-    p1 ⪯ ^ ( j ; P1 ; P2 ) p2.
-  Proof.
-    destruct p1 as [[e1 H1] rho1]; destruct p2 as [[e2 H2] rho2].
-    intros Hpre Hleq v1 c1 m1 Hleq' Hstep.
-    edestruct (Hpre v1 c1) as [v2 [c2 [m2 [Hstep2 [Hleq2 H3]]]]]; eauto.
-    omega. do 3 eexists; repeat split; eauto.
-    rewrite cc_approx_val_eq in *. eapply cc_approx_val_monotonic; eauto. omega.
-  Qed.
   
-  (** The environment relations are monotonic in the step index *)
+  (** The value relation is monotonic in the step index *)
+  Lemma cc_approx_val_monotonic (k m : nat) (P : GInv) (r1 r2 : res) :
+    r1 ≺ ^ (k; P) r2 ->
+    m <= k ->
+    r1 ≺ ^ (m; P) r2.
+  Proof.
+    revert m P r1 r2. induction k as [k IHk] using lt_wf_rec1.
+    intros m P r1 r2 Hyp Hrel.
+    destruct k as [ | k ];
+    destruct r1 as [[l1 | lf1 f1] H1]; destruct r2 as [[l2 | lf2 f2] H2]; simpl;
+    try (now intros; contradiction).
+    - destruct Hyp as [c [vs1 [vs2 [Hget1 [Hget2 Hall]]]]];
+      repeat eexists; eauto. destruct m; eauto. omega.
+    - destruct Hyp
+        as (rho1 & B1 & lf2 & f2 & v_env & rho2 & B2 & Hget & Hgetl2 & Hgetlf2  & Hyp');
+      do 7 eexists; split; [ | split; [| split ] ]; (try now eauto);
+      intros xs1 ft e1 rho1' vs1 vs2 j Hfind Hlen Hset;
+      destruct (Hyp' xs1 ft e1 rho1' vs1 vs2 j Hfind Hlen Hset)
+        as (xs2 & e2 & rho2' & Hfind' & Hset' & HT);
+      do 3 eexists; repeat split; try now eauto.
+      intros. omega.
+    - destruct Hyp as [c [vs1 [vs2 [Hget1 [Hget2 Hall]]]]];
+      repeat eexists; eauto.
+      destruct m; [ now eauto | ]. eapply Forall2_monotonic; [| eassumption ].
+      intros. rewrite cc_approx_val_eq in *. eapply IHk; [| eassumption |]; omega. 
+    - destruct Hyp
+        as (rho1 & B1 & lf2 & f2 & v_env & rho2 & B2 & Hget & Hgetl2 & Hgetlf2 & Hyp');
+      do 7 eexists; split; [ | split; [| split ] ]; (try now eauto);
+      intros xs1 ft e1 rho1' vs1 vs2 j Hfind Hlen Hset;
+      destruct (Hyp' xs1 ft e1 rho1' vs1 vs2 j Hfind Hlen Hset)
+        as (xs2 & e2 & rho2' & Hfind' & Hset' & Hi);
+      do 3 eexists; repeat split; try now eauto.
+      intros Hlt' HH Hall; intros.
+      eapply Hi; eauto. omega.
+  Qed.
+
+  Section IndMon.
+
+    Variable (P1 : Inv).
+    Variable (P2 : GInv).
+
+    (** The invariants are antimonotonic in the step index *)
+    Variable (InvIndMon : forall n m, m <= n -> inclusion _ (P1 n) (P1 m)).
+    Variable (GInvIndMon : forall n m, m <= n -> inclusion _ (P1 n) (P1 m)).
+
+    (** The expression relation is anti-monotonic in the step index *)
+    Lemma cc_approx_exp_monotonic (k j : nat) p1 p2 :
+      p1 ⪯ ^ ( k ; P1 ; P2 ) p2 ->
+      j <= k ->
+      p1 ⪯ ^ ( j ; P1 ; P2 ) p2.
+    Proof.
+      destruct p1 as [[e1 H1] rho1]; destruct p2 as [[e2 H2] rho2].
+      intros Hpre Hleq H1' H2' v1 c1 m1 HH1 HH2 Hleq' Hstep.
+      edestruct (Hpre H1' H2' v1 c1)
+        as [v2 [c2 [m2 [Hstep2 [Hleq2 H3]]]]]; eauto.
+      omega. do 3 eexists; repeat split; eauto.
+      eapply InvIndMon; [| eassumption ]. omega.
+      rewrite cc_approx_val_eq in *.
+      eapply cc_approx_val_monotonic; eauto. omega.
+    Qed.
+  End IndMon.
+
+  (** The environment relations are anti-monotonic in the step index *)
   Lemma cc_approx_env_P_monotonic (R : Ensemble var) (k j : nat) (P : GInv)
         c1 c2 :
     c1 ⋞ ^ ( R ; k ; P ) c2 ->
@@ -423,9 +458,10 @@ Module CC_log_rel (H : Heap).
     destruct c1 as [H1 rho1]; destruct c2 as [H2 rho2].
     intros Hcc Hleq x HP v Hget.
     edestruct Hcc as [v2 [Heq Hpre2]]; eauto.
-    eexists; split; eauto. eapply cc_approx_val_monotonic; eauto.
+    eexists; split; eauto.
+    eapply cc_approx_val_monotonic; eauto.
   Qed.
-
+  
   Lemma cc_approx_env_monotonic (k j : nat) (P : GInv) c1 c2 :
     cc_approx_env k P c1 c2 ->
     j <= k ->
@@ -433,7 +469,7 @@ Module CC_log_rel (H : Heap).
   Proof.
     intros Hleq H. eapply cc_approx_env_P_monotonic; eauto.
   Qed.
-
+  
   (** * Proper Instances *)
 
   Global Instance cc_approx_env_proper_set :
@@ -461,7 +497,7 @@ Module CC_log_rel (H : Heap).
     destruct c1 as [H1 rho1]; destruct c2 as [H2 rho2].
     intros Hpre1 Hpre2 x HP2. inv HP2; eauto.
   Qed.
-
+  
   Lemma cc_approx_env_P_inter_l (P1 P2 : Ensemble var) (k : nat) (P : GInv) c1 c2 :
     c1 ⋞ ^ ( P1 ; k ; P ) c2 ->
     c1 ⋞ ^ ( P1 :&: P2 ; k ; P ) c2.
@@ -478,50 +514,49 @@ Module CC_log_rel (H : Heap).
     intros Hpre x HP2. inv HP2; eauto.
   Qed.
   
-  
   (** * Preservation under enviroment extension lemmas *)
 
-  Lemma cc_approx_var_env_extend_eq :
-    forall  (k : nat) (P : GInv) (rho1 rho2 : env) (H1 H2 : heap val)
-       (x y : var) (l1 l2 : loc),
-      (l1, H1) ≺ ^ (k; P) (l2, H2) ->
-      cc_approx_var_env k P H1 (M.set x l1 rho1) H2 (M.set y l2 rho2) x y.
+  Lemma cc_approx_var_env_set_eq :
+    forall (k : nat) (P : GInv) (rho1 rho2 : env) (H1 H2 : heap block)
+      (x y : var) (v1 v2 : value),
+      (v1, H1) ≺ ^ (k; P) (v2, H2) ->
+      cc_approx_var_env k P H1 (M.set x v1 rho1) H2 (M.set y v2 rho2) x y.
   Proof.
     intros rho1 rho2 H1 H2 k P x y v1 v2 Hval x' Hget.
     rewrite M.gss in Hget. inv Hget. eexists.
     rewrite M.gss. split; eauto.
   Qed.
   
-  Lemma cc_approx_var_env_extend_neq :
-    forall (k : nat) (P : GInv)  (rho1 rho2 : env) (H1 H2 : heap val)
-      (x1 x2 y1 y2 : var) (l1 l2 : loc),
+  Lemma cc_approx_var_env_set_neq :
+    forall (k : nat) (P : GInv)  (rho1 rho2 : env) (H1 H2 : heap block)
+      (x1 x2 y1 y2 : var) (v1 v2 : value),
       cc_approx_var_env k P H1 rho1 H2 rho2 y1 y2 ->
       y1 <> x1 -> y2 <> x2 ->
-      cc_approx_var_env k P H1 (M.set x1 l1 rho1) H2 (M.set x2 l2 rho2) y1 y2.
+      cc_approx_var_env k P H1 (M.set x1 v1 rho1) H2 (M.set x2 v2 rho2) y1 y2.
   Proof. 
     intros k P rho1 rho2 H1 H2 x1 x2 y1 y2 v1 v2 Hval Hneq Hneq' x' Hget.
     rewrite M.gso in *; eauto.
   Qed.
-   
-  Lemma cc_approx_var_env_extend :
-    forall (k : nat) (P : GInv)  (rho1 rho2 : env) (H1 H2 : heap val)
-      (x y : var) (l1 l2 : loc),
+  
+  Lemma cc_approx_var_env_set :
+    forall (k : nat) (P : GInv)  (rho1 rho2 : env) (H1 H2 : heap block)
+      (x y : var) (v1 v2 : value),
       cc_approx_var_env k P H1 rho1 H2 rho2 y y ->
-      (l1, H1) ≺ ^ (k; P) (l2, H2) ->
-      cc_approx_var_env k P H1 (M.set x l1 rho1) H2 (M.set x l2 rho2) y y.
+      (v1, H1) ≺ ^ (k; P) (v2, H2) ->
+      cc_approx_var_env k P H1 (M.set x v1 rho1) H2 (M.set x v2 rho2) y y.
   Proof.
     intros k P rho1 rho2 H1 H2 x y v1 v2 Hvar Hval.
     destruct (peq y x); subst.
-    - apply cc_approx_var_env_extend_eq; eauto.
-    - apply cc_approx_var_env_extend_neq; eauto.
+    - apply cc_approx_var_env_set_eq; eauto.
+    - apply cc_approx_var_env_set_neq; eauto.
   Qed.
-
+  
   (** Extend the related environments with a single point *)
-  Lemma cc_approx_env_P_extend (S : Ensemble var) (k : nat) (P : GInv)
-        (rho1 rho2 : env) (H1 H2 : heap val) x l1 l2 :
+  Lemma cc_approx_env_P_set (S : Ensemble var) (k : nat) (P : GInv)
+        (rho1 rho2 : env) (H1 H2 : heap block) (x : var) (v1 v2 : value) :
       (H1, rho1) ⋞ ^ ( S \\ [set x] ; k ; P ) (H2, rho2) ->
-      (l1, H1) ≺ ^ (k; P) (l2, H2) ->
-      (H1, M.set x l1 rho1) ⋞ ^ ( S; k ; P ) (H2, M.set x l2 rho2).
+      (v1, H1) ≺ ^ (k; P) (v2, H2) ->
+      (H1, M.set x v1 rho1) ⋞ ^ ( S; k ; P ) (H2, M.set x v2 rho2).
   Proof.
     intros Henv Hval x' HP v1' Hget.
     rewrite M.gsspec in Hget. destruct (peq x' x); subst.
@@ -533,16 +568,16 @@ Module CC_log_rel (H : Heap).
   
   (** Extend the related environments with a list *)
   Lemma cc_approx_env_P_setlist_l (S : Ensemble var) (k : nat) (P : GInv)
-        (rho1 rho2 rho1' rho2' : env) (H1 H2 : heap val) xs ls1 ls2 :
+        (rho1 rho2 rho1' rho2' : env) (H1 H2 : heap block) xs (vs1 vs2 : list value) :
     (H1, rho1) ⋞ ^ ( S \\ (FromList xs) ; k ; P ) (H2, rho2) ->
-    Forall2 (fun l1 l2 => (l1, H1) ≺ ^ (k; P) (l2, H2)) ls1 ls2 ->
-    setlist xs ls1 rho1 = Some rho1' ->
-    setlist xs ls2 rho2 = Some rho2' ->
+    Forall2 (fun v1 v2 => (v1, H1) ≺ ^ (k; P) (v2, H2)) vs1 vs2 ->
+    setlist xs vs1 rho1 = Some rho1' ->
+    setlist xs vs2 rho2 = Some rho2' ->
     (H1, rho1') ⋞ ^ ( S ; k ; P ) (H2, rho2').
   Proof.
     intros Hcc Hall Hset1 Hset2 x HP v Hget.
     destruct (in_dec var_dec x xs).
-    - edestruct (@setlist_Forall2_get loc) as [v1 [v2 [Hget1 [Hget2 HP']]]];
+    - edestruct (@setlist_Forall2_get value) as [v1 [v2 [Hget1 [Hget2 HP']]]];
       try eassumption.
       rewrite Hget in Hget1. inv Hget1. repeat eexists; eauto.
     - erewrite <- setlist_not_In in Hget; eauto.
@@ -551,53 +586,11 @@ Module CC_log_rel (H : Heap).
       erewrite <- setlist_not_In; eauto.
   Qed.
 
-  (** * Getlist lemmas *)
-  
-  Lemma cc_approx_var_env_getlist (k : nat) (P : GInv)
-        (rho1 rho2 : env) (H1 H2 : heap val) xs ys ls1 :
-    Forall2 (cc_approx_var_env k P H1 rho1 H2 rho2) xs ys ->
-    getlist xs rho1 = Some ls1 ->
-    exists ls2,
-      getlist ys rho2 = Some ls2 /\
-      Forall2 (fun l1 l2 => (l1, H1) ≺ ^ (k; P) (l2, H2)) ls1 ls2.
-  Proof.
-    revert ys ls1. induction xs as [| x xs IHxs]; intros ys ls1 Hall Hget.
-    - destruct ys; inv Hall. inv Hget. eexists. split; simpl; eauto.
-    - simpl in Hget.
-      destruct (M.get x rho1) eqn:Heq1; try discriminate.
-      destruct (getlist xs rho1) eqn:Heq2; try discriminate. inv Hget.
-      destruct ys as [| y ys]; inv Hall. 
-      destruct (IHxs ys l0 H6 eq_refl) as [vs2 [Hget HAll]].
-      destruct (H4 _ Heq1) as [v2 [Heq Hpre]].
-      eexists. split; simpl; eauto. rewrite Hget, Heq. eauto.
-  Qed.
-
-  Lemma cc_approx_env_P_getlist_l (S : Ensemble var) (k : nat) (P : GInv)
-        (rho1 rho2 : env) (H1 H2 : heap val) (xs : list var) (ls1 : list loc) :
-    (H1, rho1) ⋞ ^ ( S ; k ; P ) (H2, rho2) ->
-    (FromList xs) \subset S ->
-    getlist xs rho1 = Some ls1 ->
-    exists ls2,
-      getlist xs rho2 = Some ls2 /\
-      Forall2 (fun l1 l2 => (l1, H1) ≺ ^ (k; P) (l2, H2)) ls1 ls2.
-  Proof.
-    intros Henv. revert ls1.
-    induction xs as [| x xs IHxs]; intros ls1 Hp Hget.
-    - inv Hget. eexists. split; simpl; eauto.
-    - simpl in Hget. destruct (M.get x rho1) eqn:Heq1; try discriminate.
-      destruct (getlist xs rho1) eqn:Heq2; try discriminate. inv Hget.
-      edestruct (IHxs l0) as  [vs2 [Hget HAll]]; eauto.
-      + intros x' Hin. eapply Hp. constructor 2; eauto.
-      + eapply Henv in Heq1. destruct Heq1 as [v2 [Hyp1 Hyp2]].
-        eexists. split; simpl; eauto. rewrite Hyp1. rewrite Hget.
-        constructor. apply Hp. now constructor.
-  Qed.
-
   Lemma cc_approx_env_P_set_not_in_P_l (S : Ensemble var) (k : nat) (P : GInv)
-        (rho1 rho2 : env) (H1 H2 : heap val) (x : var) (l : loc) :
+        (rho1 rho2 : env) (H1 H2 : heap block) (x : var) (v : value) :
     (H1, rho1) ⋞ ^ ( S ; k ; P ) (H2, rho2) ->
     ~ x \in S ->
-    (H1, M.set x l  rho1) ⋞ ^ ( S; k ; P ) (H2, rho2).
+    (H1, M.set x v rho1) ⋞ ^ ( S; k ; P ) (H2, rho2).
   Proof. 
     intros Hcc Hnin y Py v' Hget.
     edestruct Hcc as [v'' [Hget' Happrox]]; eauto.
@@ -605,12 +598,12 @@ Module CC_log_rel (H : Heap).
     - contradiction.
     - rewrite M.gso in Hget; eauto.
   Qed.
-
+  
   Lemma cc_approx_env_P_set_not_in_P_r (S : Ensemble var) (k : nat) (P : GInv)
-        (rho1 rho2 : env) (H1 H2 : heap val) (x : var) (l : loc) :
+        (rho1 rho2 : env) (H1 H2 : heap block) (x : var) (v : value) :
     (H1, rho1) ⋞ ^ ( S ; k ; P ) (H2, rho2) ->
     ~ x \in S ->
-    (H1, rho1) ⋞ ^ ( S; k ; P ) (H2, M.set x l rho2).
+    (H1, rho1) ⋞ ^ ( S ; k ; P ) (H2, M.set x v rho2).
   Proof. 
     intros Hcc Hnin y Py v' Hget.
     edestruct Hcc as [v'' [Hget' Happrox]]; eauto.
@@ -620,209 +613,874 @@ Module CC_log_rel (H : Heap).
     - eauto.
   Qed.
   
+  (** * The logical relation respects heap equality *)
+
+  Lemma cc_approx_val_heap_eq (k : nat) (P : GInv) (H1 H2 H1' H2' : heap block)
+        (v1 v2 : value) :
+    (v1, H1) ≺ ^ (k; P) (v2, H2) ->
+    reach' H1 [set (val_loc v1)] |- H1 ≡ H1' ->
+    reach' H2 [set (val_loc v2)] |- H2 ≡ H2' ->
+    (v1, H1') ≺ ^ (k; P) (v2, H2').
+  Proof with now eauto with Ensembles_DB.
+    revert P H1 H2 H1' H2' v1 v2. induction k as [k IHk] using lt_wf_rec1.
+    intros P H1 H2 H1' H2' v1 v2 Hyp Heq1 Heq2.
+    destruct k as [ | k ];
+    destruct v1 as [l1 | lf1 f1]; destruct v2 as [l2 | lf2 f2];
+    try (now intros; contradiction).
+    - destruct Hyp as [c [vs1 [vs2 [Hget1 [Hget2 Hall]]]]].
+      rewrite Heq1 in Hget1; [| now apply reach'_extensive ].
+      repeat eexists; eauto.
+      rewrite <- Heq2; [ eassumption | now apply reach'_extensive ].
+    - destruct Hyp
+        as (rho1 & B1 & lf2 & f2 & v_env & rho2 & B2 & Hget & Hgetl2 & Hgetlf2 & Hyp').
+      rewrite Heq1 in Hget; [| now apply reach'_extensive ].
+      do 7 eexists; split; [ | split; [| split] ]; (try now eauto).
+      rewrite <- Heq2; [ eassumption | now apply reach'_extensive ].
+      rewrite <- Heq2; [ eassumption | ].
+      rewrite reach_unfold. right. eapply reach'_extensive.
+      repeat eexists; eauto. simpl. rewrite FromList_cons...
+      intros xs1 ft e1 rho1' vs1 vs2 j Hfind Hlen Hset;
+      destruct (Hyp' xs1 ft e1 rho1' vs1 vs2 j Hfind Hlen Hset)
+        as (xs2 & e2 & rho2' & Hfind' & Hset' & Hi).
+      do 3 eexists; repeat split; try now eauto.
+    - destruct Hyp as [c [vs1 [vs2 [Hget1 [Hget2 Hall]]]]].
+      rewrite Heq1 in Hget1; [| now apply reach'_extensive ].
+      repeat eexists; eauto.
+      rewrite <- Heq2; [ eassumption | now apply reach'_extensive ].
+      eapply Forall2_monotonic_strong; [| eassumption ].
+      intros. rewrite cc_approx_val_eq in *. eapply IHk; try eassumption.
+      omega.
+      eapply heap_eq_antimon; [| eassumption ]. rewrite (reach_unfold _ [set l1]).
+      eapply Included_Union_preserv_r. eapply reach'_set_monotonic.
+      eapply Singleton_Included. repeat eexists; eauto. simpl.
+      rewrite Heq1; [ eassumption | now apply reach'_extensive ].
+      simpl. rewrite FromList_map_image_FromList. now eexists; split; eauto.
+      eapply heap_eq_antimon; [| eassumption ]. rewrite (reach_unfold _ [set l2]).
+      eapply Included_Union_preserv_r. eapply reach'_set_monotonic.
+      eapply Singleton_Included. repeat eexists; eauto. simpl.
+      rewrite FromList_map_image_FromList. now eexists; split; eauto.
+    - destruct Hyp
+        as (rho1 & B1 & lf2 & f2 & v_env & rho2 & B2 & Hget & Hgetl2 & Hgetlf2 & Hyp').
+      rewrite Heq1 in Hget; [| now apply reach'_extensive ].
+      do 7 eexists; split; [ | split; [| split] ]; (try now eauto).
+      rewrite <- Heq2; [ eassumption | now apply reach'_extensive ].
+      rewrite <- Heq2; [ eassumption | ].
+      rewrite reach_unfold. right. eapply reach'_extensive.
+      repeat eexists; eauto. simpl. rewrite FromList_cons...
+      intros xs1 ft e1 rho1' vs1 vs2 j Hfind Hlen Hset;
+      destruct (Hyp' xs1 ft e1 rho1' vs1 vs2 j Hfind Hlen Hset)
+        as (xs2 & e2 & rho2' & Hfind' & Hset' & Hi).
+      do 3 eexists; repeat split; try now eauto.
+      assert (Hr1 : reach' H1 (env_locs rho1 (occurs_free_fundefs B1)) |- H1 ≡ H1').
+      { eapply heap_eq_antimon; [| eassumption ].
+        rewrite (reach_unfold _ [set lf1]). eapply Included_Union_preserv_r.
+        eapply reach'_set_monotonic. intros l1 Henv.
+        repeat eexists; try eassumption.
+        rewrite Heq1; [ eassumption | now apply reach'_extensive ].
+        eassumption. }
+      assert (Hr2 : reach' H2 (env_locs rho2 (occurs_free_fundefs B2)) |- H2 ≡ H2').
+      { eapply heap_eq_antimon; [| eassumption ].
+        rewrite (reach_unfold _ [set l2]). eapply Included_Union_preserv_r.
+        rewrite (reach_unfold _ (post H2 [set l2])).
+        eapply Included_Union_preserv_r. eapply reach'_set_monotonic.
+        intros l1 Henv. 
+        repeat eexists; try eassumption. simpl. rewrite FromList_cons... }
+      intros Hlt H1'' H2'' HH1 HH2. eapply Hi. omega.
+      rewrite <- reach'_heap_eq in HH1; try eassumption.
+      eapply Equivalence_Transitive; eassumption.
+      rewrite <- reach'_heap_eq in HH2; try eassumption.
+      eapply Equivalence_Transitive; eassumption.
+  Qed.
+
+  Lemma cc_approx_var_env_heap_eq (k : nat) (P : GInv)
+        (H1 H2 H1' H2' : heap block) (rho1 rho2 : env) (x y : var):
+    cc_approx_var_env k P H1 rho1 H2 rho2 x y ->
+    reach' H1 (env_locs rho1 [set x]) |- H1 ≡ H1' ->
+    reach' H2 (env_locs rho2 [set y]) |- H2 ≡ H2' ->
+    cc_approx_var_env k P H1' rho1 H2' rho2 x y.
+  Proof.
+    intros Henv Heq1 Heq2 v Hget.
+    edestruct Henv as [v2 [Hget' Hval]]; eauto.
+    eexists; split; eauto. eapply cc_approx_val_heap_eq.
+    eassumption.
+    eapply heap_eq_antimon; [| eassumption ].
+    eapply reach'_set_monotonic. eapply Singleton_Included.
+    eexists; split; eauto. rewrite Hget. reflexivity.
+    eapply heap_eq_antimon; [| eassumption ].
+    eapply reach'_set_monotonic. eapply Singleton_Included.
+    eexists; split. eauto. rewrite Hget'. reflexivity.
+  Qed.
+
+  Lemma cc_approx_env_P_heap_eq (S : Ensemble var) (k : nat) (P : GInv)
+        (H1 H2 H1' H2' : heap block) (rho1 rho2 : env) :
+    (H1, rho1) ⋞ ^ (S; k; P) (H2, rho2) ->
+    reach' H1 (env_locs rho1 S) |- H1 ≡ H1' ->
+    reach' H2 (env_locs rho2 S) |- H2 ≡ H2' ->
+    (H1', rho1) ⋞ ^ (S; k; P) (H2', rho2).
+  Proof.
+    intros Henv Heq1 Heq2 x HS v Hget.
+    edestruct Henv as [l2 [Hget' Hval]]; eauto.
+    eexists; split; eauto. eapply cc_approx_val_heap_eq.
+    eassumption.
+    eapply heap_eq_antimon; [| eassumption ].
+    eapply reach'_set_monotonic. eapply Singleton_Included.
+    eexists; split; eauto. rewrite Hget. reflexivity.
+    eapply heap_eq_antimon; [| eassumption ].
+    eapply reach'_set_monotonic. eapply Singleton_Included.
+    eexists; split. eassumption. rewrite Hget'. reflexivity.
+  Qed.
+    
+  (** * Preservation under allocation lemmas *)
+  
+  Lemma cc_approx_val_alloc_Vconstr_set (k : nat) (P : GInv)
+        (H1 H2 H1' H2' : heap block) (v1 v2 : value) (l1 l2 : loc)
+        (c : cTag) (vs1 vs2 : list value) :
+    well_formed (reach' H1 [set (val_loc v1)]) H1 ->
+    (val_loc v1) \in dom H1 ->
+    well_formed (reach' H2 [set (val_loc v2)]) H2 ->
+    (val_loc v2) \in dom H2 ->
+    (v1, H1)  ≺ ^ (k; P) (v2, H2) ->
+    alloc (Vconstr c vs1) H1 = (l1, H1') ->
+    alloc (Vconstr c vs2) H2 = (l2, H2') ->
+    Forall2 (fun v1 v2 => (v1, H1) ≺ ^ (k - 1; P) (v2, H2)) vs1 vs2 ->
+    (v1, H1')  ≺ ^ (k; P) (v2, H2').
+  Proof with now eauto with Ensembles_DB.
+    revert P H1 H2 H1' H2' v1 v2. induction k as [k IHk] using lt_wf_rec1.
+    intros P H1 H2 H1' H2' v1 v2 Hwf1 Hsub1 Hwf2 Hsub2 Hyp Ha1 Ha2 Hall.
+    destruct k as [ | k ];
+    destruct v1 as [l1' | lf1 f1]; destruct v2 as [l2' | lf2 f2];
+    try (now intros; contradiction).
+    - destruct Hyp as [c' [vs1' [vs2' [Hget1 [Hget2 Hall']]]]].
+      repeat eexists; eauto; erewrite gao; eauto.
+      intros Hc; subst. erewrite alloc_fresh in Hget1; eauto. congruence.
+      intros Hc; subst. erewrite alloc_fresh in Hget2; eauto. congruence.
+    - destruct Hyp
+        as (rho1 & B1 & lf2 & f2 & v_env & rho2 & B2 & Hget & Hgetl2 & Hgetlf2 & Hyp').
+      do 7 eexists; split; [ | split; [| split] ]; (try now eauto).
+      erewrite gao; try eassumption.
+      intros Hc; subst. erewrite alloc_fresh in Hget; eauto. congruence.
+      erewrite gao; try eassumption.
+      intros Hc; subst. erewrite alloc_fresh in Hgetl2; eauto. congruence.
+      erewrite gao; try eassumption.
+      intros Hc; subst. erewrite alloc_fresh in Hgetlf2; eauto. congruence.
+      intros xs1 ft e1 rho1' vs3 vs4 j Hfind Hlen Hset;
+      destruct (Hyp' xs1 ft e1 rho1' vs3 vs4 j Hfind Hlen Hset)
+        as (xs2 & e2 & rho2' & Hfind' & Hset' & Hi).
+      do 3 eexists; repeat split; try now eauto.
+    - destruct Hyp as [c' [vs1' [vs2' [Hget1 [Hget2 Hall']]]]].
+      repeat eexists; try eassumption; try erewrite gao; eauto.
+      intros Hc; subst. erewrite alloc_fresh in Hget1; eauto. congruence.
+      intros Hc; subst. erewrite alloc_fresh in Hget2; eauto. congruence.
+      eapply Forall2_monotonic_strong; [| eassumption ].
+      intros. rewrite cc_approx_val_eq in *.
+      eapply IHk; try eassumption.
+      + omega.
+      + eapply well_formed_antimon; [| eassumption ].
+        rewrite (reach_unfold _ [set val_loc (Loc l1')]).
+        eapply Included_Union_preserv_r.
+        eapply reach'_set_monotonic. eapply Singleton_Included.
+        repeat eexists; eauto. simpl. rewrite FromList_map_image_FromList.
+        eapply In_image. eassumption.
+      + eapply Hwf1; [| now apply Hget1 |].
+        eapply reach'_extensive. reflexivity.
+        simpl. rewrite FromList_map_image_FromList.
+        eexists; split; eauto.
+      + eapply well_formed_antimon; [| eassumption ].
+        rewrite (reach_unfold _ [set val_loc (Loc l2')]).
+        eapply Included_Union_preserv_r.
+        eapply reach'_set_monotonic. eapply Singleton_Included.
+        repeat eexists; eauto. simpl. rewrite FromList_map_image_FromList.
+        eexists; split; eauto.
+      + eapply Hwf2; [| now apply Hget2 |].
+        eapply reach'_extensive. reflexivity.
+        simpl. rewrite FromList_map_image_FromList.
+        eapply In_image. eassumption.
+      + eapply Forall2_monotonic; [| eassumption ]. intros.
+        eapply cc_approx_val_monotonic. now apply H4. omega.
+    - destruct Hyp
+        as (rho1 & B1 & lf2 & f2 & v_env  & rho2 & B2 & Hget & Hgetl2 & Hgetlf2 & Hyp').
+      do 7 eexists; split; [ | split; [| split] ]; (try now eauto).
+      erewrite gao; try eassumption.
+      intros Hc; subst. erewrite alloc_fresh in Hget; eauto. congruence.
+      erewrite gao; try eassumption.
+      intros Hc; subst. erewrite alloc_fresh in Hgetl2; eauto. congruence.
+      erewrite gao; try eassumption.
+      intros Hc; subst. erewrite alloc_fresh in Hgetlf2; eauto. congruence.
+      intros xs1 ft e1 rho1' vs3 vs4 j Hfind Hlen Hset;
+      destruct (Hyp' xs1 ft e1 rho1' vs3 vs4 j Hfind Hlen Hset)
+        as (xs2 & e2 & rho2' & Hfind' & Hset' & Hi).
+      do 3 eexists; repeat split; try now eauto.
+      intros Hlt H1'' H2'' HH1 HH2. eapply Hi.
+      + omega.
+      + eapply Equivalence_Transitive; try eassumption.
+        * eapply heap_eq_antimon; [|  eapply subheap_heap_eq ].
+          eapply reachable_in_dom. eassumption.
+          eapply Singleton_Included.
+          now repeat eexists; eauto. eapply alloc_subheap. eassumption.
+        * eapply heap_eq_antimon; [| eassumption ].
+          eapply reach'_heap_monotonic. eapply alloc_subheap. eassumption.
+      + eapply Equivalence_Transitive.
+        * eapply heap_eq_antimon; [|  eapply subheap_heap_eq ].
+          eapply reachable_in_dom. eassumption.
+          eapply Singleton_Included.
+          now repeat eexists; eauto. eapply alloc_subheap. eassumption.
+        * eapply heap_eq_antimon; [| eassumption ].
+          eapply reach'_heap_monotonic. eapply alloc_subheap. eassumption.
+  Qed.
+  
+  (** * Getlist lemmas *)
+  
+  Lemma cc_approx_var_env_getlist (k : nat) (P : GInv)
+        (rho1 rho2 : env) (H1 H2 : heap block) xs ys vs1 :
+    Forall2 (cc_approx_var_env k P H1 rho1 H2 rho2) xs ys ->
+    getlist xs rho1 = Some vs1 ->
+    exists vs2,
+      getlist ys rho2 = Some vs2 /\
+      Forall2 (fun v1 v2 => (v1, H1) ≺ ^ (k; P) (v2, H2)) vs1 vs2.
+  Proof.
+    revert ys vs1. induction xs as [| x xs IHxs]; intros ys vs1 Hall Hget.
+    - destruct ys; inv Hall. inv Hget. eexists. split; simpl; eauto.
+    - simpl in Hget.
+      destruct (M.get x rho1) eqn:Heq1; try discriminate.
+      destruct (getlist xs rho1) eqn:Heq2; try discriminate. inv Hget.
+      destruct ys as [| y ys]; inv Hall. 
+      destruct (IHxs ys l H6 eq_refl) as [vs2 [Hget HAll]].
+      destruct (H4 _ Heq1) as [v2 [Heq Hpre]].
+      eexists. split; simpl; eauto. rewrite Hget, Heq. eauto.
+  Qed.
+  
+  Lemma cc_approx_env_P_getlist_l (S : Ensemble var) (k : nat) (P : GInv)
+        (rho1 rho2 : env) (H1 H2 : heap block) (xs : list var) (vs1 : list value) :
+    (H1, rho1) ⋞ ^ ( S ; k ; P ) (H2, rho2) ->
+    (FromList xs) \subset S ->
+    getlist xs rho1 = Some vs1 ->
+    exists vs2,
+      getlist xs rho2 = Some vs2 /\
+      Forall2 (fun v1 v2 => (v1, H1) ≺ ^ (k; P) (v2, H2)) vs1 vs2.
+  Proof.
+    intros Henv. revert vs1.
+    induction xs as [| x xs IHxs]; intros ls1 Hp Hget.
+    - inv Hget. eexists. split; simpl; eauto.
+    - simpl in Hget. destruct (M.get x rho1) eqn:Heq1; try discriminate.
+      destruct (getlist xs rho1) eqn:Heq2; try discriminate. inv Hget.
+      edestruct (IHxs l) as  [vs2 [Hget HAll]]; eauto.
+      + intros x' Hin. eapply Hp. constructor 2; eauto.
+      + eapply Henv in Heq1. destruct Heq1 as [v2 [Hyp1 Hyp2]].
+        eexists. split; simpl; eauto. rewrite Hyp1. rewrite Hget.
+        constructor. apply Hp. now constructor.
+  Qed.
+  
   (** * Compatibility lemmas *)
 
-  Open Scope fun_scope.
-  
-  Lemma live_collect S H1 H2 :
-    live S H1 H2 ->
-    collect S H1 H2.
-  Proof.
-    firstorder.
-  Qed.
 
-  Definition HInv := relation nat.
+  (** TODO move *)
+  Definition AppClo f t xs f' Γ :=
+    Eproj f' clo_tag 0%N f
+          (Eproj Γ clo_tag 1%N f
+                 (Eapp f' t (Γ :: xs))).
 
-  Lemma cc_approx_exp_constr_compat (k : nat) (P : GInv) (P1 P2 : Inv) (Ph : HInv)
-        rho1 rho2 H1 H2 x1 x2 t ys1 ys2 e1 e2 :
-    Forall2 (cc_approx_var_env k P H1 rho1 H2 rho2) ys1 ys2 ->
-    (* Cost invariant compatibility property *)
-    (forall c1 m1 m1' c2 m2 m2',
-       P1 (c1, m1) (c2, m2) ->
-       Ph m1' m2' ->
-       P2 (c1 + 1 + length ys1, max m1 m1') (c2 + 1 + length ys1, max m2 m2')) ->
-    Ph (size_heap H1 + (1 + length ys1)) (size_heap H2 + (1 + length ys1)) ->
-    (forall ls1 ls2 l1 l2 H1' H2' H1'' H2'',
-       (* allocate a new location for the constructed value *)
-       alloc (Vconstr t ls1) H1 = (l1, H1') ->
-       alloc (Vconstr t ls2) H2 = (l2, H2') ->
-       (* garbage collect *)
-       reach' H1' (env_locs (M.set x1 l1 rho1) (occurs_free e1)) |- H1' ≡ H1'' ->
-       reach' H2' (env_locs (M.set x2 l2 rho2) (occurs_free e2)) |- H2' ≡ H2'' ->
-       Forall2 (fun l1 l2 => (l1, H1) ≺ ^ (k; P) (l2, H2)) ls1 ls2 ->
-       (e1, M.set x1 l1 rho1, H1'') ⪯ ^ (k ; P1; P) 
-       (e2, M.set x2 l2 rho2, H2'')) ->
-    (Econstr x1 t ys1 e1, rho1, H1) ⪯ ^ (k ; P2; P) (Econstr x2 t ys2 e2, rho2, H2).
-  Proof.
-    intros Hall Hyp Hi Hpre v1 c1 m1 Hleq1 Hstep1. inv Hstep1.
-    edestruct (cc_approx_var_env_getlist k P rho1 rho2) as [ls2 [Hget' Hpre']];
-      [| eauto |]; eauto.
-    destruct (alloc (Vconstr t ls2) H2) as [l' H2'] eqn:Ha.
-    edestruct (live_exists (env_locs (M.set x2 l' rho2) (occurs_free e2)) H2') as [H2'' Hl2].
-    eapply Decidable_env_locs; eauto with typeclass_instances.
-    eapply Forall2_length in Hall. rewrite Hall.
-    edestruct Hpre as [v2 [c2 [m2 [Hstep [HS Hval]]]]];
-      [ eassumption | eassumption | | | eassumption | | eassumption |  ].
-    eapply collect_heap_eq; eapply live_collect; eassumption.
-    eapply collect_heap_eq; eapply live_collect; eassumption.
-    omega.
-    repeat eexists; eauto. econstructor; eauto.
-    rewrite <- Hall. eapply Hyp. eassumption.
-    rewrite cc_approx_val_eq in *.
-    unfold size_heap. erewrite size_with_measure_alloc; [| reflexivity | eassumption ].
-    erewrite size_with_measure_alloc with (H' := H2'); [| reflexivity | eassumption ].
-    simpl. rewrite <- plus_n_O. erewrite <- getlist_length_eq; [| eassumption ].
-    replace (length ls2) with (length ys1). eassumption.
-    erewrite <- (getlist_length_eq _ ls2); [| eassumption ]. eassumption.
-    rewrite cc_approx_val_eq in *.
-    eapply cc_approx_val_monotonic. eassumption. omega.
-  Qed.
 
-  Lemma cc_approx_exp_proj_compat (k : nat) (P : GInv) (P1 P2 : Inv) (Ph : HInv)
-        rho1 rho2 H1 H2 x1 x2 t n y1 y2 e1 e2 :
-    cc_approx_var_env k P H1 rho1 H2 rho2 y1 y2 ->
-    (* Cost invariant compatibility property *)
-    (forall c1 m1 m1' c2 m2 m2',
-       P1 (c1, m1) (c2, m2) ->
-       Ph m1' m2' ->
-       P2 (c1 + 1, max m1 m1') (c2 + 1, max m2 m2')) ->
-    Ph (size_heap H1) (size_heap H2) ->
-    (forall i l1 l2 H1' H2',
-       i <= k ->
-       (* garbage collect *)
-       reach' H1 (env_locs (M.set x1 l1 rho1) (occurs_free e1)) |- H1 ≡ H1' ->
-       reach' H2 (env_locs (M.set x2 l2 rho2) (occurs_free e2)) |- H2 ≡ H2' ->
-       (l1, H1) ≺ ^ (i; P) (l2, H2) ->
-       (e1, M.set x1 l1 rho1, H1') ⪯ ^ (i ; P1; P) 
-       (e2, M.set x2 l2 rho2, H2')) ->
-    (Eproj x1 t n y1 e1, rho1, H1) ⪯ ^ (k ; P2; P) (Eproj x2 t n y2 e2, rho2, H2).
-  Proof.
-    intros Hall Hyp Hi Hpre r1 c1 m1 Hleq1 Hstep1. inv Hstep1.
-    edestruct Hall as [l2 [Hget' Hcc']]; eauto.
-    simpl in Hcc'. rewrite H10 in Hcc'. destruct (get l2 H2) eqn:Hget2; try contradiction.
-    destruct v; try contradiction. destruct Hcc' as [Heq Hcc']. subst.
-    destruct k; try omega.
-    edestruct (Forall2_nthN (fun l1 l2 => cc_approx_val k P (l1, H1) (l2, H2)) ls)
-      as [l2' [Hnth Hval]]; eauto.
-    edestruct (live_exists (env_locs (M.set x2 l2' rho2) (occurs_free e2)) H2)
-      as [H2' Hl2].
-    eapply Decidable_env_locs; eauto with typeclass_instances.
-    edestruct Hpre with (i := k) as [r2 [c2 [m2 [Hstep [HS Hres]]]]];
-      [omega | | | | | eassumption |].
-    eapply collect_heap_eq; eapply live_collect; eassumption.
-    eapply collect_heap_eq; eapply live_collect; eassumption.
-    rewrite cc_approx_val_eq in *.
-    eapply cc_approx_val_monotonic. eassumption. omega.
-    omega.
-    repeat eexists; eauto. econstructor; eauto.
-    rewrite cc_approx_val_eq in *.
-    eapply cc_approx_val_monotonic. eassumption. omega.
-  Qed.
-  
-  Import ListNotations.
+  Section Compat.
 
-  Lemma cc_approx_exp_case_nil_compat (k : nat) (P : GInv) (P1 P2 : Inv) (Ph : HInv)
-        rho1 rho2 H1 H2 x1 x2 :
-    (Ecase x1 [], rho1, H1) ⪯ ^ (k ; P2; P) (Ecase x2 [], rho2, H2).
-  Proof.
-    intros v1 c1 m1 Hleq1 Hstep1. inv Hstep1. inv H6.
-  Qed.
-  
+    Variable (IG : GInv). (* Global Invariant *)
+    Variable (IL1 IL2 IL: Inv). (* Local Invariants *)
+    Variable (II : IInv). (* Initial Invariant *)
 
-  Lemma cc_approx_exp_case_compat (k : nat) (P : GInv) (P1 P2 P3 : Inv) (Ph : HInv)
-        rho1 rho2 H1 H2 x1 x2 t e1 e2 Pats1 Pats2 :
+    (** The initial invariant should respect heap equality *)
+    Variable
+      (InitInvRespectsHeapEq :
+         forall (H1 H2 H1' H2' : heap block) (rho1 rho2 : env) (e1 e2 : exp),
+           reach' H1 (env_locs rho1 (occurs_free e1)) |- H1 ≡ H1' ->
+           reach' H2 (env_locs rho2 (occurs_free e2)) |- H2 ≡ H2' ->
+           II (H1, rho1, e1) (H2, rho2, e2) ->
+           II (H1', rho1, e1) (H2', rho2, e2)).
     
-    cc_approx_var_env k P H1 rho1 H2 rho2 x1 x2 ->
+    (** * Compatibility properties for the local invariants *)
     
-    (* Cost invariant compatibility properties *)
-    (forall c1 m1 m1' c2 m2 m2',
-       P1 (c1, m1) (c2, m2) ->
-       Ph m1' m2' ->
-       P3 (c1 + 1, max m1 m1') (c2 + 1, max m2 m2')) ->
-    inclusion  _ P2 P3 ->
+    (** Constructor compatibility *)
+    Variable
+      (InvConstrCompat :
+         forall (H1 H2 H1' H2' H1'' H2'': heap block) (rho1 rho2 : env)
+           (x1 x2 : var) (t : cTag) (ys1 ys2 : list var) (e1 e2 : exp)
+           (c1 c2 m1 m2 c k i : nat) (l1 l2 : loc) (b1 b2 : block),
 
-    Ph (size_heap H1) (size_heap H2) ->
+           alloc b1 H1 = (l1, H1') ->
+           live (env_locs (M.set x1 (Loc l1) rho1) (occurs_free e1)) H1' H1'' ->
 
-    (forall i H1' H2',
-       i < k ->
-       (* garbage collect *)
-       reach' H1 (env_locs rho1 (occurs_free e1)) |- H1 ≡ H1' ->
-       reach' H2 (env_locs rho2 (occurs_free e2)) |- H2 ≡ H2' ->
-       (e1, rho1, H1') ⪯ ^ (i ; P1; P) (e2, rho2, H2')) ->
+           alloc b2 H2 = (l2, H2') ->
+           live (env_locs (M.set x2 (Loc l2) rho2) (occurs_free e2)) H2' H2'' ->
 
-    (Ecase x1 Pats1, rho1, H1) ⪯ ^ (k ; P2; P) (Ecase x2 Pats2, rho2, H2) ->
+           i < k ->
+           
+           IL1 i (H1'', M.set x1 (Loc l1) rho1, e1, c1, m1) (H2'', M.set x2 (Loc l2) rho2, e2, c2, m2) -> 
 
-    (Ecase x1 ((t, e1) :: Pats1), rho1, H1) ⪯ ^ (k ; P3; P) (Ecase x2 ((t, e2) :: Pats2), rho2, H2).
-  Proof.
-    intros Hap Hyp1 Hyp2 Hyp3 Hexp_hd Hexp_tl r1 c1 m1 Hleq1 Hstep1.
-    inv Hstep1.
-    edestruct Hap as [l2 [Hget' Hcc']]; eauto.
-    simpl in Hcc'. rewrite H5 in Hcc'.
-    destruct (get l2 H2) eqn:Hget2; try contradiction.
-    destruct v; try contradiction. destruct Hcc' as [Heq Hcc'].
-    subst. destruct k; try omega.
-    simpl in H6. destruct (peq t c0); subst.
-    - rewrite peq_true in H6. inv H6.
-      edestruct (live_exists (env_locs rho2 (occurs_free e2)) H2)
-        as [H2' Hl2].
-      eapply Decidable_env_locs; typeclasses eauto.
-      edestruct Hexp_hd with (i := k) as [v2 [c2 [m2 [Hstep2 [HS Hpre2]]]]];
-        [| | | | eassumption | ].
-      omega.
-      eapply collect_heap_eq; eapply live_collect; eassumption.
-      eapply collect_heap_eq; eapply live_collect; eassumption.
-      omega. 
-      repeat eexists. econstructor; eauto; try now constructor; eauto.
-      simpl. rewrite peq_true. reflexivity.
-      eapply Hyp1. eassumption. rewrite <- plus_n_O. eassumption.
-      rewrite cc_approx_val_eq in *.
-      eapply cc_approx_val_monotonic. eassumption. omega.
-    - rewrite peq_false in H6; eauto. 
-      edestruct Hexp_tl as [v2 [c2 [m2 [Hstep2 [HS Hpre2]]]]];
-        [eassumption | now econstructor; eauto | ]. inv Hstep2.
-      repeat eexists.
-      + econstructor; eauto. simpl. rewrite peq_false. eassumption.
-        rewrite H8 in Hget'; inv Hget'. rewrite H9 in Hget2; inv Hget2.
+           II (H1, rho1, Econstr x1 t ys1 e1) (H2, rho2, Econstr x2 t ys2 e2) ->
+
+           IL k (H1, rho1, Econstr x1 t ys1 e1, c1 + c, max m1 (size_heap H1 + c))
+              (H2, rho2, Econstr x2 t ys2 e2, c2 + c, max m2 (size_heap H2 + c))).
+
+    (** Projection compatibility *)
+    Variable
+      (InvProjCompat :
+         forall (H1 H2 H1' H2' : heap block) (rho1 rho2 : env)
+           (x1 x2 : var) (t : cTag) (n : N) (y1 y2 : var) (e1 e2 : exp)
+           (c1 c2 m1 m2 c k i : nat) (v1 v2 : value),
+
+           live (env_locs (M.set x1 v1 rho1) (occurs_free e1)) H1 H1' ->
+
+           live (env_locs (M.set x2 v2 rho2) (occurs_free e2)) H2 H2' ->
+
+           i < k ->
+
+           IL1 i (H1', M.set x1 v1 rho1, e1, c1, m1) (H2', M.set x2 v2 rho2, e2, c2, m2) -> 
+
+           II (H1, rho1, Eproj x1 t n y1 e1) (H2, rho2, Eproj x2 t n y2 e2) ->
+
+           IL k (H1, rho1, Eproj x1 t n y1 e1, c1 + c, max m1 (size_heap H1))
+              (H2, rho2, Eproj x2 t n y2 e2, c2 + c, max m2 (size_heap H2))).
+
+    (** Case compatibility *)
+    Variable
+      (InvCaseHdCompat :
+         forall (H1 H2 H1' H2' : heap block) (rho1 rho2 : env)
+           (y1 y2 : var) (t : cTag) (e1 e2 : exp) (P1 P2 : list (cTag * exp))
+           (c1 c2 m1 m2 c i k : nat),
+
+           live (env_locs rho1 (occurs_free e1)) H1 H1' ->
+
+           live (env_locs rho2 (occurs_free e2)) H2 H2' ->
+
+           i < k ->
+
+           IL1 i (H1', rho1, e1, c1, m1) (H2', rho2, e2, c2, m2) -> 
+
+           II (H1, rho1, Ecase y1 ((t, e1) :: P1)) (H2, rho2, Ecase y2 ((t, e2) :: P2)) ->
+
+           IL k (H1, rho1, Ecase y1 ((t, e1) :: P1), c1 + c, max m1 (size_heap H1))
+              (H2, rho2, Ecase y2 ((t, e2) :: P2), c2 + c, max m2 (size_heap H2))).
+
+    Variable
+      (InvCaseTlCompat :
+         forall (H1 H2 : heap block) (rho1 rho2 : env)
+           (y1 y2 : var) (t : cTag) (e1 e2 : exp) (P1 P2 : list (cTag * exp))
+           (c1 c2 m1 m2 c k : nat),
+            
+           IL2 k (H1, rho1, Ecase y1 P1, c1 + c, m1)
+               (H2, rho2, Ecase y2 P2, c2 + c, m2) -> 
+
+           II (H1, rho1, Ecase y1 ((t, e1) :: P1)) (H2, rho2, Ecase y2 ((t, e2) :: P2)) ->
+
+           IL k (H1, rho1, Ecase y1 ((t, e1) :: P1), c1 + c, m1)
+              (H2, rho2, Ecase y2 ((t, e2) :: P2), c2 + c, m2)).
+
+    (** Halt compatibility *)
+    Variable
+      (InvHaltCompat :
+         forall (H1 H2 : heap block) (rho1 rho2 : env)
+           (x1 x2 : var) (c k : nat),
+
+           II (H1, rho1, Ehalt x1) (H2, rho2, Ehalt x2) ->
+
+           IL k (H1, rho1, Ehalt x1, c, size_heap H1) (H2, rho2, Ehalt x2, c, size_heap H2)).
+    
+    (** App compatibility *)
+    (* Messy compat assumption :( *)
+    Variable
+      (InvAppCompat :
+         forall (H1 H2 H1' H2' : heap block)
+           (rho1 rho2 rho1' rho2' rho1'' rho2'' : env)
+           (f1 f2 f1' f2' f2'' Γ : var) (t : cTag) (xs1 xs2 ys1 ys2 : list var) (e1 e2 : exp)
+           (B1 B2 : fundefs) (lf1 lc2 lf2 : loc) (venv : value)
+           (c1 c2 m1 m2 c i k : nat) (vs1 vs2 : list value),
+           
+           M.get f1 rho1 = Some (FunPtr lf1 f1') ->
+           get lf1 H1 = Some (Vfun rho1' B1) ->
+           getlist xs1 rho1 = Some vs1 ->
+           find_def f1' B1 = Some (t, ys1, e1) ->
+           setlist ys1 vs1 (def_funs B1 lf1 rho1') = Some rho1'' ->
+           live (env_locs rho1'' (occurs_free e1)) H1 H1' ->
+
+           M.get f2 rho2 = Some (Loc lc2) ->
+           get lc2 H2 = Some (Vconstr clo_tag [(FunPtr lf2 f2') ; venv]) ->
+           get lf2 H2 = Some (Vfun rho2' B2) ->
+           getlist xs2 rho2 = Some vs2 ->
+           find_def f2' B2 = Some (t, ys2, e2) ->
+           setlist ys2 (venv :: vs2) (def_funs B2 lf2 rho2') = Some rho2'' ->
+           live (env_locs rho1'' (occurs_free e1)) H1 H1' ->
+
+           i < k ->
+
+           IG i (H1', rho1'', e1, c1, m1) (H2', rho2'', e2, c2, m2) -> 
+           
+           II (H1, rho1, Eapp f1 t xs1) (H2, rho2, AppClo f2 t xs2 f2'' Γ) ->
+
+           IL k (H1, rho1, Eapp f1 t xs1, c1 + c, max m1 (size_heap H1))
+              (H2, rho2, AppClo f2 t xs2 f2'' Γ, c2 + c + 3, max m2 (size_heap H2))).
+
+    (** Abstraction compatibility *)
+    Variable
+      (InvFunCompat :
+         forall (H1 H2 H1' H2' H1'' H2'': heap block) (rho1 rho2 : env)
+           (B1 B2 : fundefs) (e1 e2 : exp) (c1 c2 m1 m2 s c k i : nat) (l1 l2 : loc),
+
+           alloc (Vfun rho1 B1) H1 = (l1, H1') ->
+           live (env_locs (def_funs B1 l1 rho1) (occurs_free e1)) H1' H1'' ->
+           
+           alloc (Vfun rho2 B2) H2 = (l2, H2') ->
+           live (env_locs (def_funs B2 l2 rho2) (occurs_free e2)) H2' H2'' ->
+
+           i < k ->
+
+           IL1 i (H1'', def_funs B1 l1 rho1, e1, c1, m1) (H2'', def_funs B2 l2 rho2, e2, c2, m2) -> 
+           
+           II (H1, rho1, Efun B1 e1) (H2, rho2, Efun B2 e2) ->
+
+           IL k (H1, rho1, Efun B1 e1, c1 + fundefs_num_fv B1 + c, max m1 (size_heap H1 + s))
+              (H2, rho2, Efun B2 e2, c2 + fundefs_num_fv B2 + c, max m2 (size_heap H2 + s))).
+
+    (** Constructor compatibility *)
+    Lemma cc_approx_exp_constr_compat (k : nat)
+          rho1 rho2 H1 H2 x1 x2 t ys1 ys2 e1 e2 :
+
+      Forall2 (cc_approx_var_env k IG H1 rho1 H2 rho2) ys1 ys2 ->
+
+      II (H1, rho1, Econstr x1 t ys1 e1) (H2, rho2, Econstr x2 t ys2 e2) ->
+      
+      (forall i vs1 vs2 l1 l2 H1' H2' H1'' H2'',
+         i < k ->
+         (* quantify over all equal heaps *)
+         reach' H1 (env_locs rho1 (occurs_free (Econstr x1 t ys1 e1))) |- H1 ≡ H1' ->
+         reach' H2 (env_locs rho2 (occurs_free (Econstr x2 t ys2 e2))) |- H2 ≡ H2' ->
+                                                                                                                                         (* allocate a new location for the constructed value *)
+                                                                                                                                           alloc (Vconstr t vs1) H1' = (l1, H1'') ->
+                                                                                                                                           alloc (Vconstr t vs2) H2' = (l2, H2'') ->
+                                                                                                                                           Forall2 (fun l1 l2 => (l1, H1') ≺ ^ (i; IG) (l2, H2')) vs1 vs2 ->
+                                                                                                                                           (e1, M.set x1 (Loc l1) rho1, H1'') ⪯ ^ (i; IL1; IG)
+          (e2, M.set x2 (Loc l2) rho2, H2'')) ->
+      
+      (Econstr x1 t ys1 e1, rho1, H1) ⪯ ^ (k; IL; IG) (Econstr x2 t ys2 e2, rho2, H2).
+    Proof with now eauto with Ensembles_DB.
+      intros Hall Hinit Hpre H1' H2' v1 c1 m1 Heq1 Heq2 Hleq1 Hstep1.
+      inv Hstep1.
+      edestruct (cc_approx_var_env_getlist k IG rho1 rho2) as [ls2 [Hget' Hpre']];
+        [| eauto |]; eauto.
+      destruct (alloc (Vconstr t ls2) H2') as [l' H2''] eqn:Ha.
+      edestruct (live_exists (env_locs (M.set x2 (Loc l') rho2) (occurs_free e2)) H2'')
+        as [H2''' Hl2].
+      eapply Decidable_env_locs; eauto with typeclass_instances.
+      eapply Forall2_length in Hall. rewrite Hall.
+      assert (Hlen : @length M.elt ys1 = @length M.elt ys2).
+      { erewrite (@getlist_length_eq value ys1 vs); [| eassumption ].
+        erewrite (@getlist_length_eq value ys2 ls2); [| eassumption ].
+        eapply Forall2_length. eassumption. }
+      edestruct Hpre with (i := k - (1 + @length M.elt ys2)) as [v2 [c2 [m2 [Hstep [HS Hval]]]]];
+        [ |  eassumption | eassumption | eassumption | eassumption | | | | | eassumption | ].
+      - omega.
+      - eapply Forall2_monotonic_strong; [| eassumption ]. intros ? ? ? ? H.
+        eapply cc_approx_val_monotonic.
+        eapply cc_approx_val_heap_eq. now apply H.
+        eapply heap_eq_antimon; [| eassumption ]. eapply reach'_set_monotonic.
+        eapply Singleton_Included. eapply FromList_env_locs. eassumption.
+        normalize_occurs_free... rewrite FromList_map_image_FromList.
+        eapply In_image; eassumption.
+        eapply heap_eq_antimon; [| eassumption ]. eapply reach'_set_monotonic.
+        eapply Singleton_Included. eapply FromList_env_locs. eassumption.
+        normalize_occurs_free... rewrite FromList_map_image_FromList.
+        eapply In_image; eassumption. omega.
+      - eapply collect_heap_eq. eapply live_collect. eassumption.
+      - eapply collect_heap_eq. eapply live_collect. eassumption.
+      - rewrite <- Hlen. eapply NPeano.Nat.le_add_le_sub_r. rewrite plus_assoc.
+        eassumption. (* Because of type mismatch, omega does not solve this *) 
+      - repeat eexists; eauto.
+        + now econstructor; eauto.
+        + rewrite <- Hall, <- plus_n_O.
+          unfold size_heap. 
+          erewrite (size_with_measure_alloc _ _ _ H1' H'); [| reflexivity | eassumption ].
+          erewrite size_with_measure_alloc with (H' := H2''); [| reflexivity | eassumption ].
+          simpl. replace (c + 1 + length ys1) with (c + S (length ys1)) by omega.
+          replace (c2 + 1 + length ys1) with (c2 + S (length ys1)) by omega.
+          erewrite <- (getlist_length_eq ys1 vs); [| eassumption ].
+          replace (length ls2) with (length ys1).
+          eapply InvConstrCompat; try eassumption. omega. 
+          eapply InitInvRespectsHeapEq; eassumption.
+          erewrite <- (getlist_length_eq _ ls2); [| eassumption ]. eassumption.
+        + replace (k - (c + 1 + length ys2)) with (k - (1 + length ys2) - c) by omega.
+          eassumption.
+    Qed.
+
+    (** Projection compatibility *)
+    Lemma cc_approx_exp_proj_compat (k : nat) rho1 rho2 H1 H2 x1 x2 t n y1 y2 e1 e2 :
+
+      cc_approx_var_env k IG H1 rho1 H2 rho2 y1 y2 ->
+
+      II (H1, rho1, Eproj x1 t n y1 e1) (H2, rho2, Eproj x2 t n y2 e2) ->
+
+      (forall i v1 v2 H1' H2',
+         i < k ->
+         (* quantify over all equal heaps *)
+         reach' H1 (env_locs rho1 (occurs_free (Eproj x1 t n y1 e1))) |- H1 ≡ H1' ->
+         reach' H2 (env_locs rho2 (occurs_free (Eproj x2 t n y2 e2))) |- H2 ≡ H2' ->
+                                                                                                                                          (v1, H1) ≺ ^ (i; IG) (v2, H2) ->
+                                                                                                                                          (e1, M.set x1 v1 rho1, H1') ⪯ ^ (i ; IL1; IG) (e2, M.set x2 v2 rho2, H2')) ->
+      
+      (Eproj x1 t n y1 e1, rho1, H1) ⪯ ^ (k ; IL; IG) (Eproj x2 t n y2 e2, rho2, H2).
+    Proof.
+      intros Hall Hi Hpre H1' H2' r1 c1 m1 Heq1' Heq2' Hleq1 Hstep1. inv Hstep1.
+      edestruct Hall as [l2 [Hget' Hcc']]; eauto.
+      destruct l2 as [l' | l' f]; [| contradiction ].
+      destruct Hcc' as [c' [vs1 [vs2 [Hget1 [Hget2' Hk]]]]].
+      rewrite Heq1' in Hget1; [
+        | now eapply reach'_extensive; repeat eexists; eauto; rewrite H7; eauto ].
+      rewrite Heq2' in Hget2'; [
+        | now eapply reach'_extensive; repeat eexists; eauto; rewrite Hget'; eauto ]. 
+      rewrite Hget1 in H10; inv H10.
+      destruct k; try omega.
+      edestruct (Forall2_nthN (fun l1 l2 => cc_approx_val k IG (l1, H1) (l2, H2)) vs)
+        as [l2' [Hnth Hval]]; eauto.
+      edestruct (live_exists (env_locs (M.set x2 l2' rho2) (occurs_free e2)) H2')
+        as [H2'' Hl2].
+      eapply Decidable_env_locs; eauto with typeclass_instances.
+      edestruct Hpre with (i := k) as [r2 [c2 [m2 [Hstep [HS Hres]]]]];
+        [omega | eassumption | eassumption | | | | | eassumption | ].
+      - rewrite cc_approx_val_eq in *.
         eassumption.
-      + eapply Hyp2. rewrite <- plus_n_O in *. eassumption.
-      + rewrite cc_approx_val_eq in *.
+      - eapply collect_heap_eq. eapply live_collect. eassumption.
+      - eapply collect_heap_eq. eapply live_collect. eassumption.
+      - omega.
+      - repeat eexists; eauto. now econstructor; eauto.
+        rewrite cc_approx_val_eq in *.
         eapply cc_approx_val_monotonic. eassumption. omega.
-  Qed.
+    Qed.
+
+    (** Case compatibility *)
+    Lemma cc_approx_exp_case_nil_compat (k : nat) rho1 rho2 H1 H2 x1 x2 :
+      (Ecase x1 [], rho1, H1) ⪯ ^ (k ; IL; IG) (Ecase x2 [], rho2, H2).
+    Proof.
+      intros H1' H2' v1 c1 m1 Hleq1 Hstep1 Hleq Hstep. inv Hstep.
+      inv H6.
+    Qed.
   
-  Lemma cc_approx_exp_halt_compat (k : nat) (P : GInv) (P1 : Inv) (Ph : HInv)
-        rho1 rho2 H1 H2 x1 x2 :
-    cc_approx_var_env k P H1 rho1 H2 rho2 x1 x2 ->
-    (forall m1 m2, Ph m1 m2 -> P1 (1, m1) (1, m2)) ->
-    Ph (size_heap H1) (size_heap H2) ->
-    (Ehalt x1, rho1, H1) ⪯ ^ (k ; P1; P) (Ehalt x2, rho2, H2).
-  Proof.
-    intros Henv Hc Hi v1 c1 m1 Hleq1 Hstep1. inv Hstep1.
-    edestruct Henv as [v' [Hget Hpre]]; eauto.
-    repeat eexists; eauto. now econstructor; eauto.
-    rewrite cc_approx_val_eq in *.
-    eapply cc_approx_val_monotonic. eassumption. omega.
-  Qed.
+    Lemma cc_approx_exp_case_compat (k : nat) rho1 rho2 H1 H2 x1 x2 t e1 e2 Pats1 Pats2 :
+      
+      cc_approx_var_env k IG H1 rho1 H2 rho2 x1 x2 ->
 
-  Lemma cc_approx_exp_app_compat (k : nat) (P : GInv) (P1 : Inv) (Ph : HInv)
-        rho1 rho2 H1 H2 t f1 xs1 f2 f2' Γ xs2 :
-    cc_approx_var_env k P H1 rho1 H2 rho2 f1 f2 ->
-    Forall2 (cc_approx_var_env k P H1 rho1 H2 rho2) xs1 xs2 ->
-    (forall m1 m2, Ph m1 m2 -> P1 (1 + length xs1, m1) (1 + length xs1, m2)) ->
-    Ph (size_heap H1) (size_heap H2) ->
-    (Eapp f1 t xs1, rho1, H1) ⪯ ^ (k ; P1; P)
-    (Eproj f2' clo_tag 0%N f2
-           (Eproj Γ clo_tag 1%N f2
-                  (Eapp f2' t (Γ :: xs2))), rho2, H2).
-  Proof.
-    intros Henv Hall Hc Hi v1 c1 m1 Hleq1 Hstep1. inv Hstep1.
-    edestruct Henv as [l' [Hget' Hcc']]; eauto.
-    edestruct (cc_approx_var_env_getlist k P rho1 rho2) as [ls2 [Hgetl' Hcc'']];
-      [| eauto |]; eauto.
-    simpl in Hcc'. rewrite H6 in Hcc'.
-    destruct (get l' H2) eqn:Hget2; try contradiction.
-    destruct v; try contradiction. destruct l0; try contradiction.
-    destruct l1; try contradiction.
-    destruct Hcc' as [rho2' [B' [Hget HallB]]].
-  Abort.
+      II (H1, rho1, Ecase x1 ((t, e1) :: Pats1)) (H2, rho2, Ecase x2 ((t, e2) :: Pats2)) ->
 
-End  CC_log_rel.
+      (forall i H1' H2',
+         i < k ->
+         (* quantify over all equal heaps *)
+         reach' H1 (env_locs rho1 (occurs_free (Ecase x1 ((t, e1) :: Pats1)))) |- H1 ≡ H1' ->
+         reach' H2 (env_locs rho2 (occurs_free (Ecase x2 ((t, e2) :: Pats2)))) |- H2 ≡ H2' ->
+
+         (e1, rho1, H1') ⪯ ^ (i ; IL1; IG) (e2, rho2, H2')) ->
+
+      (Ecase x1 Pats1, rho1, H1) ⪯ ^ (k ; IL2; IG) (Ecase x2 Pats2, rho2, H2) ->
+
+      (Ecase x1 ((t, e1) :: Pats1), rho1, H1) ⪯ ^ (k ; IL; IG) (Ecase x2 ((t, e2) :: Pats2), rho2, H2).
+    Proof with now eauto with Ensembles_DB.
+      intros Hap HI Hexp_hd Hexp_tl H1' H2' r1 c1 m1 Heq1 Heq2 Hleq1 Hstep1.
+      inv Hstep1.
+      edestruct Hap as [l2 [Hget' Hcc']]; eauto.
+      destruct l2 as [l' |l' f ]; [| contradiction ].
+      destruct Hcc' as [c' [vs1 [vs2 [Hget1 [Hget2' Hk]]]]].
+      rewrite Heq1 in Hget1; [
+        | now eapply reach'_extensive; repeat eexists; eauto; rewrite H4; eauto ].
+      rewrite Heq2 in Hget2'; [
+        | now eapply reach'_extensive; repeat eexists; eauto; rewrite Hget'; eauto ]. 
+      rewrite Hget1 in H5; inv H5.
+      destruct k; try omega.
+      simpl in H6. destruct (peq t t0); subst.
+      - rewrite peq_true in H6. inv H6.
+        edestruct (live_exists (env_locs rho2 (occurs_free e2)) H2')
+          as [H2'' Hl2].
+        eapply Decidable_env_locs; typeclasses eauto.
+        edestruct Hexp_hd with (i := k) as [v2 [c2 [m2 [Hstep2 [HS Hpre2]]]]];
+          [| eassumption | eassumption | | | | eassumption | ].
+        + omega.
+        + eapply collect_heap_eq; eapply live_collect; eassumption.
+        + eapply collect_heap_eq; eapply live_collect; eassumption.
+        + omega. 
+        + repeat eexists; eauto.
+          * econstructor; eauto; try now constructor; eauto.
+            simpl. rewrite peq_true. reflexivity.
+          * rewrite cc_approx_val_eq in *.
+            eapply cc_approx_val_monotonic. eassumption. omega.
+      - rewrite peq_false in H6; eauto. 
+        edestruct Hexp_tl as [v2 [c2 [m2 [Hstep2 [HS Hpre2]]]]];
+          [ | |  eassumption | now econstructor; eauto | ].
+        + eapply heap_eq_antimon; [| eassumption ].
+          eapply reach'_set_monotonic. eapply env_locs_monotonic.
+          normalize_occurs_free...
+        + eapply heap_eq_antimon; [| eassumption ].
+          eapply reach'_set_monotonic. eapply env_locs_monotonic.
+          normalize_occurs_free...
+        + inv Hstep2. repeat eexists; eauto.
+          * econstructor; eauto. simpl.
+            rewrite peq_false. eassumption.
+            rewrite H5 in Hget'; inv Hget'. rewrite H8 in Hget2'; inv Hget2'.
+            eassumption.
+          * rewrite <- plus_n_O in *; eauto.
+    Qed.
+
+    (** Halt compatibility *)
+    Lemma cc_approx_exp_halt_compat (k : nat) rho1 rho2 H1 H2 x1 x2 :
+      cc_approx_var_env k IG H1 rho1 H2 rho2 x1 x2 ->
+
+      II (H1, rho1, Ehalt x1) (H2, rho2, Ehalt x2) ->
+
+      (Ehalt x1, rho1, H1) ⪯ ^ (k ; IL; IG) (Ehalt x2, rho2, H2).
+    Proof.
+      intros Henv Hi H1' H2' v1 c1 m1 Heq1 Heq2 Hleq1 Hstep1. inv Hstep1.
+      edestruct Henv as [v' [Hget Hpre]]; eauto.
+      repeat eexists.
+      - now econstructor; eauto.
+      - rewrite <- plus_n_O in *; eauto.
+      - rewrite cc_approx_val_eq in *.
+        eapply cc_approx_val_heap_eq.
+        eapply cc_approx_val_monotonic. eassumption.
+        omega.
+        eapply heap_eq_antimon; [| eassumption ].
+        eapply reach'_set_monotonic.
+        eapply Singleton_Included. repeat eexists; eauto.
+        now rewrite H3; eauto.
+        eapply heap_eq_antimon; [| eassumption ].
+        eapply reach'_set_monotonic.
+        eapply Singleton_Included. repeat eexists; eauto.
+        now rewrite Hget; eauto.
+    Qed.
+    
+    (** Application compatibility *)
+    Lemma cc_approx_exp_app_compat (k : nat) rho1 rho2 H1 H2 t f1 xs1 f2 f2' Γ xs2 :
+      ~ Γ \in (f2 |: FromList xs2) ->
+      ~ f2' \in (f2 |: FromList xs2) ->
+      Γ <> f2' ->
+      cc_approx_var_env k IG H1 rho1 H2 rho2 f1 f2 ->
+      Forall2 (cc_approx_var_env k IG H1 rho1 H2 rho2) xs1 xs2 ->
+      II (H1, rho1, Eapp f1 t xs1) (H2, rho2, AppClo f2 t xs2 f2' Γ)  ->
+      (Eapp f1 t xs1, rho1, H1) ⪯ ^ (k ; IL; IG) (AppClo f2 t xs2 f2' Γ, rho2, H2).
+    Proof with now eauto with Ensembles_DB.
+      intros Hnin1 Hnin2 Hneq Henv Hall Hi H1' H2' v1 c1 m1 Heq1 Heq2 Hleq1 Hstep1.
+      inv Hstep1.
+      (* weaken the hypotheses *)
+      eapply cc_approx_var_env_heap_eq in Henv;
+        try now (eapply heap_eq_antimon; [| eassumption ];
+                 eapply reach'_set_monotonic; eapply env_locs_monotonic;
+                 eapply Singleton_Included; eauto).
+      eapply Forall2_monotonic_strong in Hall;
+        [| intros ? ? ? ? Hval;
+           eapply cc_approx_var_env_heap_eq; [ now apply Hval | |];
+           (eapply heap_eq_antimon; [| eassumption ]);
+           eapply reach'_set_monotonic; eapply env_locs_monotonic;
+           eapply Singleton_Included; eauto
+        ].
+      - edestruct Henv as [l' [Hget' Hcc']]; eauto. unfold AppClo in *.
+        edestruct (cc_approx_var_env_getlist k IG rho1 rho2) as [vs2 [Hgetl' Hcc'']];
+          [| now eauto |]; eauto.
+        simpl in Hcc'. destruct l' as [l' | ]; [| contradiction ]. 
+        destruct Hcc'
+          as (rho1' & B1 & lf2 & f2'' & venv & rho2' & B2 & Hgetl & Hgetl'' & Hgetlf & HBs).
+        rewrite Hgetl in H6; inv H6.
+        edestruct HBs with (j := k - 1) (vs1 := vs) (vs2 := vs2)
+          as (xs2' & e2 & rho2'' & Hf2'' & Hset & Hj); eauto.
+        eapply Forall2_length. eassumption.
+        (* first GC *)
+        edestruct (live_exists (env_locs (M.set f2' (FunPtr lf2 f2'') rho2)
+                                         (occurs_free (Eproj Γ clo_tag 1 f2 (Eapp f2' t (Γ :: xs2))))) H2')
+          as [H21 Hl2].
+        eapply Decidable_env_locs; eauto with typeclass_instances.
+        (* second GC *)
+        edestruct (live_exists (env_locs (M.set Γ venv (M.set f2' (FunPtr lf2 f2'') rho2))
+                                         (occurs_free (Eapp f2' t (Γ :: xs2)))) H21)
+          as [H22 Hl2'].
+        eapply Decidable_env_locs; eauto with typeclass_instances.
+        (* third GC *)
+        edestruct (live_exists (env_locs rho2'' (occurs_free e2)) H22)
+          as [H23 Hl2''].
+        eapply Decidable_env_locs; eauto with typeclass_instances.
+        
+        assert (Hlocs_eq :
+                  reach' H2' (env_locs (M.set Γ venv (M.set f2' (FunPtr lf2 f2'') rho2))
+                                       (occurs_free (Eapp f2' t (Γ :: xs2)))) \subset
+                         reach' H2' (env_locs (M.set f2' (FunPtr lf2 f2'') rho2)
+                                              (occurs_free (Eproj Γ clo_tag 1 f2 (Eapp f2' t (Γ :: xs2)))))).
+        { normalize_occurs_free. rewrite !occurs_free_Eapp at 1. rewrite !FromList_cons at 1.
+          rewrite !Setminus_Union_distr, Setminus_Same_set_Empty_set, Union_Empty_set_neut_l. 
+          rewrite !Setminus_Disjoint. rewrite !env_locs_set_In; eauto. 
+          rewrite !Setminus_Union_distr, !Setminus_Same_set_Empty_set, Union_Empty_set_neut_r. 
+          rewrite (Setminus_Union [set f2'] [set Γ] [set f2']), (Union_commut [set Γ] [set f2']).
+          rewrite <- Setminus_Union, !Setminus_Same_set_Empty_set, !Setminus_Empty_set_abs_r,
+          Union_Empty_set_neut_r, Union_Empty_set_neut_l.
+          rewrite !Setminus_Disjoint, env_locs_Union, !reach'_Union.
+          rewrite (Union_assoc (reach' H2' [set val_loc venv])).
+          rewrite (Union_commut (reach' H2' [set val_loc venv])), <- Union_assoc.
+          simpl.
+          rewrite (reach_unfold _ (env_locs rho2 [set f2])).
+          rewrite !env_locs_Singleton at 1; [ | now eauto | now eauto]. simpl.
+          rewrite post_Singleton; [| now eauto ]. simpl. rewrite !FromList_cons at 1.
+          rewrite !reach'_Union...
+          eapply Disjoint_Singleton_r. intros Hc. eapply Hnin2. now right.
+          eapply Disjoint_Singleton_r. intros Hc. inv Hc. eapply Hnin2. now left.
+          eapply Disjoint_Singleton_r. intros Hc. eapply Hnin1. now right.
+          eapply Disjoint_Singleton_r. intros Hc. inv Hc. eapply Hnin2. now right.
+          constructor. now eauto. intros Hc; inv Hc; congruence.
+          eapply Disjoint_Singleton_r. intros Hc. inv Hc. congruence.
+          eapply Disjoint_Singleton_r. intros Hc. eapply Hnin1. now right. }
+        assert (Hlocs_eq' :
+                  reach' H2' (env_locs rho2'' (occurs_free e2)) \subset
+                         reach' H2' (env_locs (M.set Γ venv (M.set f2' (FunPtr lf2 f2'') rho2))
+                                              (occurs_free (Eapp f2' t (Γ :: xs2))))).
+        { normalize_occurs_free. rewrite !FromList_cons at 1.
+          rewrite !env_locs_set_In; eauto. eapply Included_trans.
+          eapply reach'_set_monotonic. eapply Included_trans.
+          eapply env_locs_monotonic.
+          eapply occurs_free_in_fun. eapply find_def_correct. eassumption.
+          eapply Included_trans.
+          rewrite Union_commut. eapply env_locs_setlist_Included. now eauto.
+          eapply Included_Union_compat. rewrite Union_commut. now eapply env_locs_def_funs_Included. 
+          simpl. rewrite FromList_cons. reflexivity. simpl.
+          rewrite !reach'_Union. eapply Union_Included.
+          eapply Union_Included. eapply Included_Union_preserv_r.
+          eapply Included_Union_preserv_l.
+          rewrite (reach'_idempotent _ [set lf2]).
+          eapply reach'_set_monotonic.
+          intros l1 Hin. exists 1. split. now constructor.
+          exists lf2. eexists; split; [ | split; try eassumption ].
+          reflexivity. now eauto with Ensembles_DB.
+          eapply Union_Included. now eauto with Ensembles_DB.
+          do 2 eapply Included_Union_preserv_r.
+          eapply reach'_set_monotonic. eapply FromList_env_locs.
+          eassumption.
+          rewrite !Setminus_Union_distr, Setminus_Same_set_Empty_set; eauto. 
+          eapply Included_Union_preserv_l. eapply Included_Union_preserv_r.
+          rewrite !Setminus_Disjoint. reflexivity.
+          eapply Disjoint_Singleton_r. intros Hc. eapply Hnin1. now right.
+          eapply Disjoint_Singleton_r. intros Hc. inv Hc. eapply Hnin2. now right.
+          constructor. now eauto. intros Hc; inv Hc. congruence. }
+        assert (Heap1 :
+                  reach' H2'
+                         (env_locs (M.set f2' (FunPtr lf2 f2'') rho2)
+                                   (occurs_free (Eproj Γ clo_tag 1 f2 (Eapp f2' t (Γ :: xs2))))) |- H2' ≡ H21).
+        { eapply collect_heap_eq; eapply live_collect; eassumption. }
+        assert (Heap2 :
+                  reach' H2'
+                         (env_locs (M.set Γ venv (M.set f2' (FunPtr lf2 f2'') rho2))
+                                   (occurs_free (Eapp f2' t (Γ :: xs2)))) |- H21 ≡ H22).
+        { eapply heap_eq_antimon; [| eapply collect_heap_eq; eapply live_collect; eassumption ].
+          rewrite reach'_heap_eq. reflexivity.
+          eapply heap_eq_antimon; [| eassumption ]. eassumption. }
+        assert (Heap3 :
+                  reach' H2' (env_locs rho2'' (occurs_free e2)) |- H22 ≡ H23).
+        { eapply heap_eq_antimon; [| eapply collect_heap_eq; eapply live_collect; eassumption ].
+          rewrite reach'_heap_eq. reflexivity.
+          eapply Equivalence_Transitive.
+          eapply heap_eq_antimon; [| eassumption ]. eapply Included_trans; eassumption.
+          eapply heap_eq_antimon; [| eassumption ]. eassumption. }
+        edestruct Hj with (H1' := H') (H2' := H23) as (r2 & c2 & m2 & Hstep & Hinv & Hval);
+          [ omega | reflexivity | reflexivity |  | | | | eassumption | ].
+        + eapply Forall2_monotonic; [| eassumption ].
+          intros ? ? Hval. rewrite !cc_approx_val_eq in *.
+          eapply cc_approx_val_monotonic. now apply Hval. omega.
+        + eapply collect_heap_eq; eapply live_collect; eassumption.
+        + eapply Equivalence_Transitive; [| eapply Equivalence_Transitive ].
+          * (* H2' = H21  *)
+            eapply heap_eq_antimon; [| eassumption ].
+            eapply Included_trans; eassumption.
+          * (* H21 = H22 *)
+            eapply heap_eq_antimon; eassumption. 
+          * (* H22 = H23 *)
+            eassumption.
+        + omega.
+        + repeat eexists.
+          * econstructor. eassumption. eassumption. reflexivity.
+            eassumption. reflexivity.
+            econstructor; eauto.
+            rewrite M.gso. eassumption. intros Hc.
+            subst. eapply Hnin2. now left; eauto.
+            rewrite <- Heap1. eassumption.
+            eapply reach'_extensive. eapply env_locs_monotonic with (S1 := [set f2]).
+            normalize_occurs_free...
+            eexists; split; eauto. rewrite M.gso. now rewrite Hget'.
+            now intros Hc; subst; eauto.
+            reflexivity.
+            econstructor. exact 0. (* XXX extra nat in the semantics *)
+            rewrite M.gso. rewrite M.gss. reflexivity.
+            now intros Hc; subst; eauto.
+            rewrite <- Heap2, <- Heap1. eassumption.
+            eapply reach'_extensive. eapply env_locs_monotonic with (S1 := [set f2']).
+            eapply Singleton_Included. repeat normalize_occurs_free.
+            right. constructor; eauto. intros Hc; inv Hc; congruence.
+            eexists; split; eauto. rewrite M.gss. reflexivity.
+            eapply reach'_extensive. eapply env_locs_monotonic with (S1 := [set f2']).
+            eapply Singleton_Included. repeat normalize_occurs_free...
+            eexists; split; eauto. rewrite M.gso. rewrite M.gss. reflexivity.
+            now eauto. simpl. rewrite M.gss.
+            rewrite !getlist_set_neq. now rewrite Hgetl'.
+            intros Hc. eapply Hnin2. now eauto.
+            intros Hc. eapply Hnin1. now eauto.
+            eassumption. now eauto. eassumption. reflexivity.
+            eassumption.
+          * rewrite <- plus_n_O. simpl.
+            replace (c2 + 1 + S (length xs2) + 1 + 1) with (c2 + (S (length xs2)) + 3) by omega.
+            replace (c + 1 + length xs1) with (c + S (length xs1)) by omega. 
+            rewrite <- !Max.max_assoc, (Max.max_r (size_heap H22)), (Max.max_r (size_heap H21)).
+            erewrite Forall2_length; eauto.
+            eapply InvAppCompat; try eassumption. now eauto. omega. now eauto.
+            eapply size_with_measure_subheap. now destruct Hl2.
+            eapply le_trans; [| now apply NPeano.Nat.le_max_l ].
+            eapply size_with_measure_subheap. now destruct Hl2'.
+          * rewrite cc_approx_val_eq in *. eapply cc_approx_val_monotonic.
+            eassumption.  omega.
+      - unfold AppClo. repeat normalize_occurs_free.
+        right. constructor. right. constructor. left.
+        rewrite FromList_cons...
+        intros Hc; inv Hc; eapply Hnin1. now right.
+        intros Hc; inv Hc; eapply Hnin2. now right.
+      - eapply heap_eq_antimon; [| eassumption ].
+        eapply reach'_set_monotonic. eapply env_locs_monotonic.
+        eapply Singleton_Included. unfold AppClo.
+        repeat normalize_occurs_free. eauto.
+    Qed.
+
+    (** Abstraction compatibility *)
+    Lemma cc_approx_exp_fun_compat (k : nat) rho1 rho2 H1 H2 B1 e1 B2 e2 :
+      II (H1, rho1, Efun B1 e1) (H2, rho2, Efun B2 e2)  ->
+      (forall i l1 l2 H1' H2' H1'' H2'',
+         i < k ->
+         (* quantify over all equal heaps *)
+         reach' H1 (env_locs rho1 (occurs_free (Efun B1 e1))) |- H1 ≡ H1' ->
+         reach' H2 (env_locs rho2 (occurs_free (Efun B2 e2))) |- H2 ≡ H2' ->
+         (* allocate a new location for the abstraction *)
+         alloc (Vfun rho1 B1) H1' = (l1, H1'') ->
+         alloc (Vfun rho2 B2) H2' = (l2, H2'') ->
+         (e1, def_funs B1 l1 rho1, H1'') ⪯ ^ (i; IL1; IG)
+         (e2, def_funs B2 l2 rho2, H2'')) ->
+      (Efun B1 e1, rho1, H1) ⪯ ^ (k ; IL; IG) (Efun B2 e2, rho2, H2).
+    Proof with now eauto with Ensembles_DB.
+      intros Hinit Hpre H1' H2' v1 c1 m1 Heq1 Heq2 Hleq1 Hstep1.
+      inv Hstep1.
+      destruct (alloc (Vfun rho2 B2) H2') as [l' H2''] eqn:Ha.
+      edestruct (live_exists (env_locs (def_funs B2 l' rho2) (occurs_free e2)) H2'')
+        as [H2''' Hl2].
+      eapply Decidable_env_locs; eauto with typeclass_instances.
+
+      edestruct Hpre with (i := k - 1) as [v2 [c2 [m2 [Hstep [HS Hval]]]]];
+        [ |  eassumption | eassumption | eassumption | eassumption | | | | eassumption | ].
+      - omega.
+      - eapply collect_heap_eq. eapply live_collect. eassumption.
+      - eapply collect_heap_eq. eapply live_collect. eassumption.
+      - omega.
+      - repeat eexists; eauto.
+        + now econstructor; eauto.
+        + rewrite <- plus_n_O.
+          unfold size_heap. 
+          erewrite (size_with_measure_alloc _ _ _ H1' H'); [| reflexivity | eassumption ].
+          erewrite size_with_measure_alloc with (H' := H2''); [| reflexivity | eassumption ].
+          eapply InvFunCompat; try eassumption.
+          omega. now eauto.
+        + rewrite cc_approx_val_eq in *.
+          eapply cc_approx_val_monotonic. eassumption. omega.
+    Qed.
+
+  End Compat.
+
+End CC_log_rel.
