theories/L6_PCPS/Heap/closure_conversion_correct.v
@@ -1,0 +1,86 @@
+From L6 Require Import cps size_cps cps_util set_util identifiers ctx Ensembles_util
+     List_util functions closure_conversion.
+
+From L6.Heap Require Import heap heap_defs space_sem cc_log_rel.
+
+From Libraries Require Import Coqlib.
+
+From Coq Require Import ZArith.Znumtheory Relations.Relations Arith.Wf_nat
+                        Lists.List MSets.MSets MSets.MSetRBT Numbers.BinNums
+                        NArith.BinNat PArith.BinPos Sets.Ensembles Omega.
+
+Import ListNotations.
+
+Open Scope ctx_scope.
+Open Scope fun_scope.
+Close Scope Z_scope.
+
+Module ClosureConversionCorrect (H : Heap).
+
+  (* Module Sem := SpaceSem H. *)
+  Module LogRel := CC_log_rel H.
+
+  Import H LogRel.Sem LogRel.Sem.Defs LogRel.
+  
+  Variable clo_tag : cTag.
+
+  Variable (IG : GInv).
+  Variable (IL1 IL2 IL : GInv).
+  
+
+  (** Correctness of [Closure_conversion] *)
+  Lemma Closure_conversion_correct (k : nat) (H1 H2 : heap block)
+        (rho1 rho2 : env) (e1 e2 : exp) (C : exp_ctx)
+        (Scope Funs : Ensemble var) (FVs : list var)
+        (σ : var -> var) (c : cTag) (Γ : var) :
+    (* [Scope] invariant *)
+    (H1, rho1) ⋞ ^ (Scope; k; IG) (H2, rho2) ->
+    (* [Fun] invariant *)
+    Fun_inv k IG rho1 H1 rho2 H2 Scope Funs σ c Γ ->
+    (* Free variables invariant *)
+    FV_inv k IG rho1 H1 rho2 H2 Scope Funs c Γ FVs ->
+    
+    (* [Γ] (the current environment parameter) is not bound in e *)
+    ~ In _ (bound_var e1) Γ ->
+    (* The free variables of e are defined in the environment *)
+    binding_in_map (occurs_free e1) rho1 ->
+    (* The blocks of functions have unique function names *)
+    fundefs_names_unique e1 ->
+    (* function renaming is injective in the [Funs] subdomain *)
+    injective_subdomain Funs σ ->
+    (* function renaming codomain is not shadowed by other vars *)
+    Disjoint _ (image σ (Setminus _ Funs Scope)) (bound_var e1) ->
+
+    (* [e'] is the closure conversion of [e] *)
+    Closure_conversion clo_tag Scope Funs σ c Γ FVs e1 e2 C ->
+    (e1, rho1, H1) ⪯ ^ (k; IL; IG) (C |[ e2 ]|, rho2, H2).
+  Proof with now eauto with Ensembles_DB.
+    revert H1 H2 rho1 rho2 e1 e2 C Scope Funs FVs σ c Γ.
+    induction k as [k IHk] using lt_wf_rec1.
+    intros H1 H2 rho1 rho2 e1 e2 C Scope Funs FVs σ c Γ
+           Henv Hnin HFVs Hun Hinj Hd Hfun Hfv Hcc.
+    induction e1 using exp_ind'; try clear IHe1.
+    - (* case Econstr *)
+      inv Hcc.
+      admit.
+    - (* case Ecase nil *)
+      inv Hcc.
+      admit.
+    - (* case Ecase cons *)
+      inv Hcc. (* TODO change compat *) 
+      admit.
+    - (* case Eproj *)
+      inv Hcc.
+      admit.
+    - (* case Efun *)
+      inv Hcc.
+      admit.
+    - (* case Eapp *)
+      inv Hcc.
+      admit.
+    - (* case Eprim *)
+      intros ? ? ? ? ? ? ? ? Hstep. inv Hstep.
+    - (* case Ehalt *)
+      inv Hcc.
+      admit.
+  Abort.
